implement keccak

Blanc.lean
@@ -5,13 +5,10 @@ partial def Bytes.chunks (bs : Bytes) : List Bytes :=
   | (_, []) => [bs]
   | (bs', bs'') => bs' :: chunks bs''
 
-def Bytes.toHexString (bs : Bytes) : String :=
-  "hex\"" ++ List.foldr (λ b s => b.toString ++ s) "\"" bs
-
 def WethByteCode : String :=
   List.foldr
      (λ s0 s1 => s0 ++ "\n" ++ s1)
-     "" <| List.map Bytes.toHexString (Option.getD weth.compile []).chunks
+     "" <| List.map Bytes.toHexString
+        <| Bytes.chunks <| Option.getD weth'.compile []
 
-def main : IO Unit :=
-  IO.println WethByteCode
+def main : IO Unit := IO.println WethByteCode
