Blanc/Basic.lean
@@ -1,12 +1,10 @@
-
-
-
 -- Basic.lean : generic definitions and lemmas (e.g. for Booleans, lists,
 -- bit vectors and bytes) that are useful for but not specific to Blanc
 
 import Mathlib.Data.Nat.Defs
 import Mathlib.Data.List.Lemmas
 import Mathlib.Util.Notation3
+import Mathlib.Data.Vector.Basic
 
 
 
@@ -19,26 +17,13 @@ def Bool.toChar : Bool → Char
   | 0 => '0'
   | 1 => '1'
 
-lemma Bool.zero_toNat : (0 : Bool).toNat = 0 := rfl
-lemma Bool.one_toNat : (1 : Bool).toNat = 1 := rfl
-
-lemma false_toNat : (false : Bool).toNat = 0 := rfl
-lemma true_toNat : (true : Bool).toNat = 1 := rfl
-
-lemma true_eq_one : true = 1 := rfl
-lemma false_eq_zero : false = 0 := rfl
-
 lemma Bool.zero_or_one (x : Bool) : x = 0 ∨ x = 1 := by
   cases x
   · left; rfl
   · right; rfl
 
-lemma not_true_lt_false : ¬ true < false := by simp [LT.lt]
 lemma not_true_lt {b} : ¬ true < b := by simp [LT.lt]
-lemma not_true_le_false : ¬ true ≤ false := by simp [LE.le]
 lemma false_lt_true : false < true := by simp [LT.lt]
-lemma false_le {b : Bool} : false ≤ b := by cases b <;> simp [LE.le]
-lemma Bool.le_one {b : Bool} : b ≤ 1 := by cases b <;> simp [LE.le]; rfl
 lemma Bool.zero : 0 = false := rfl
 lemma Bool.one : 1 = true := rfl
 
@@ -94,18 +79,6 @@ lemma List.of_cons_split {X} {x : X} {xs ys zs} (h : (x :: xs) <++ ys ++> zs) :
 lemma List.of_nil_split {X} {p p' : List X} : ([] <++ p ++> p') → p = p' := by simp [Split]
 
 universe u
-
-lemma cond_elim {ξ : Type u} (π : ξ → Prop) (b : Bool) (x y : ξ)
-    (h : b = true → π x) (h' : b = false → π y) : π (cond b x y) := by
-  cases b; apply h' rfl; apply h rfl
-
-lemma ite_cases {ξ : Sort u} (r : ξ → Prop) (c : Prop) [h : Decidable c] (x y : ξ) :
-    (c → r x) → (¬ c → r y) → r (if c then x else y) := by
-  have h : (if c then x else y) = (if c then x else y) := rfl
-  intros hx hy; rw [ite_eq_iff'] at h; rcases h with ⟨hx', hy'⟩
-  cases em c with
-  | inl h => rw [← hx' h]; apply hx h
-  | inr h => rw [← hy' h]; apply hy h
 
 lemma Nat.forall_lt_succ_iff_forall_le {n : ℕ} {p : ℕ → Prop} :
     (∀ m < (n + 1), p m) ↔ (∀ m ≤ n, p m) := by
@@ -202,20 +175,12 @@ macro_rules
 abbrev Byte := Bits 8
 
 abbrev Bytes : Type := List Byte
--- inductive Bytes : Type
---   | nil : Bytes
---   | cons : Bytes → Byte → Bytes
-
--- infixl:70 " :> " => Bytes.cons
---
--- syntax "[" withoutPosition(term,*,?) "]"  : term
--- macro_rules | `([$l,*]) => `(expand_foldl% (h t => Bytes.cons h t) Bytes.nil [$(.ofElems l),*])
 
 def Bits.toChars : ∀ {n}, Bits n → List Char
   | 0, ⦃⦄ => []
-  | _ + 1, x +> xs => x.toChar :: xs.toChars
+  | _ + 1, x +> xs => Bool.toChar x :: xs.toChars
 
-def Bits.toString {n} (bs : Bits n) : String := ⟨bs.toChars⟩
+def Bits.toString {n} (bs : Bits n) : String := ⟨Bits.toChars bs⟩
 
 instance {n} : Repr (Bits n) := ⟨λ bs _ => Bits.toString bs⟩
 
@@ -255,9 +220,6 @@ instance {n} : @LE (Bits n) := ⟨Bits.le⟩
 lemma Bits.cons_lt_cons {n} {x y} {xs ys : Bits n} :
     x +> xs < y +> ys ↔ (x < y ∨ (x = y ∧ xs < ys)) := Iff.refl _
 
--- lemma Bits.cons_lt_cons' {n} {xs ys : Bits n} {x} :
---     x +> xs < ys +> x ↔ xs < ys := by simp [cons_lt_cons]
---
 lemma Bits.cons_eq_cons {n} {x y} {xs ys : Bits n} :
     x +> xs = y +> ys ↔ (x = y ∧ xs = ys) := by simp
 
@@ -328,7 +290,8 @@ def Bits.max : ∀ n : ℕ, Bits n
 
 def Bits.one : ∀ n : ℕ, Bits n
   | 0 => ⦃⦄
-  | n + 1 => 0 +> one n
+  | 1 => ⦃1⦄
+  | n + 2 => 0 +> one (n + 1)
 
 instance {n} : @One (Bits n) := ⟨Bits.one n⟩
 
@@ -342,13 +305,6 @@ def Bits.rec2 {μ : ∀ n, Bits n → Bits n → Sort u}
     match xs, ys with
     | x +> xs, y +> ys => apply cons; apply ih
 
-  --| succ n =>
--- def Bits.carrySucc : ∀ {n}, Bits n → (Bool × Bits n)
---   | 0, ⦃⦄ => (1, ⦃⦄)
---   | _ + 1, x +> xs =>
---     let (y, ys) := xs.carrySucc
---     (x && y, (x != y) +> ys)
---
 def Bits.isMax : ∀ {n}, Bits n → Bool
   | 0, ⦃⦄ => true
   | _ + 1, x +> xs => x && xs.isMax
@@ -357,28 +313,9 @@ def Bits.succ : ∀ {n}, Bits n →  Bits n
   | 0, ⦃⦄ => ⦃⦄
   | _ + 1, x +> xs => (x != xs.isMax) +> xs.succ
 
-lemma Bits.succ_inj {n} {xs ys : Bits n} : xs.succ = ys.succ → xs = ys := by
-  apply @Bits.rec2 (λ _ xs ys => xs.succ = ys.succ → xs = ys) (λ _ => rfl)
-  intro n x xs y ys ih h; simp only [succ, cons_eq_cons] at h
-  rcases h with ⟨h, h'⟩; cases ih h';
-  rw [Bool.xor_right_inj] at h; cases h; rfl
-
-def Bits.succs {n} : Nat → Bits n → Bits n
-  | 0, xs => xs
-  | n + 1, xs => succs n xs.succ
-
 def Bits.incr {n} : Bool → Bits n → Bits n
   | false => id
   | true => Bits.succ
-
-def Bits.carryAdd : ∀ {n}, Bits n → Bits n → (Bool × Bits n)
-  | 0, ⦃⦄, ⦃⦄ => (0, ⦃⦄)
-  | _ + 1, x +> xs, y +> ys =>
-    let (z, zs) := carryAdd xs ys
-    ((x && y) || (x && z) || (y && z), ((x != y) != z) +> zs)
-
----def Bits.add {n} (xs ys : Bits n) : Bits n := (carryAdd xs ys).snd
-
 
 def Overflow {n : ℕ} (xs ys : Bits n) : Prop := 2 ^ n ≤ xs.toNat + ys.toNat
 
@@ -393,12 +330,6 @@ lemma overflow_comm :
   · intro n x xs y ys ih; simp only [overflow, bne]
     rw [Bool.and_comm, Bool.beq_comm, ih];
 
-
-
-
-
-
-
 def Bits.add : ∀ {n : ℕ}, Bits n → Bits n → Bits n
   | 0, ⦃⦄, ⦃⦄ => ⦃⦄
   | _ + 1, x +> xs, y +> ys =>
@@ -406,64 +337,12 @@ def Bits.add : ∀ {n : ℕ}, Bits n → Bits n → Bits n
 
 infix:55 " ↟ " => Overflow
 
-lemma Nat.mul_le_mul_iff {a b c : ℕ} (h : 0 < c) : c * a ≤ c * b ↔ a ≤ b := by
-  constructor <;> intro h'
-  · apply Nat.le_of_mul_le_mul_left h' h
-  · apply Nat.mul_le_mul_left _ h'
-
-lemma Nat.lt_floor_left {a b c d : ℕ} (h : d < c) : c * a + d < c * b ↔ c * a < c * b := by
-  constructor <;> intro h'
-  · apply lt_of_le_of_lt (Nat.le_add_right _ _) h'
-  · have hc : 0 < c := Nat.lt_of_le_of_lt (Nat.zero_le _) h
-    have h'' : c * a + d < c * a + c := by
-      rw [Nat.add_lt_add_iff_left]; exact h
-    apply lt_of_lt_of_le h''
-    rw [← Nat.mul_succ, Nat.mul_le_mul_iff hc, Nat.succ_le]
-    rw [Nat.mul_lt_mul_left hc] at h'; exact h'
-
-lemma Nat.eq_floor {a b c d e : ℕ} (hd : d < c) (he : e < c)
-    (h : c * a + d = c * b + e) : a = b ∧ d = e := by
-  have hc : 0 < c := Nat.lt_of_le_of_lt (Nat.zero_le _) hd
-  rcases Nat.lt_trichotomy a b with h' | h' | h'
-  · apply False.elim <| Nat.lt_irrefl (c * b) _
-    apply lt_of_le_of_lt (Nat.le_add_right (c * b) e)
-    rw [← h, Nat.lt_floor_left hd]
-    apply Nat.mul_lt_mul_of_pos_left h' hc
-  · simp [h'] at h; refine ⟨h', h⟩
-  · apply False.elim <| Nat.lt_irrefl (c * a) _
-    apply lt_of_le_of_lt (Nat.le_add_right (c * a) d)
-    rw [h, Nat.lt_floor_left he]
-    apply Nat.mul_lt_mul_of_pos_left h' hc
-
 def Nof {n : ℕ} (xs ys : Bits n) : Prop := xs.toNat + ys.toNat < 2 ^ n
 
 def Bits.nof_iff_not_overflow {n : ℕ} (xs ys : Bits n) : Nof xs ys ↔ ¬ xs ↟ ys := by
   simp [Overflow, Nof]
 
---def Bits.pred : ∀ {n}, Bits n → Bits n
---  | 0, ⦃⦄ => ⦃⦄
---  | _ + 1, xs +> 0 => xs.pred +> 1
---  | _ + 1, xs +> 1 => xs +> 0
---
---def Bits.decr {n} : Bool → Bits n → Bits n
---  | false, xs => xs
---  | true, xs => xs.pred
-
-def Bits.carrySub : ∀ {n}, Bits n → Bits n → (Bool × Bits n)
-  | 0, ⦃⦄, ⦃⦄ => (0, ⦃⦄)
-  | n + 1, x +> xs, y +> ys =>
-    let (z, zs) := carrySub xs ys
-    ((!x && (y != z)) || (y && z), ((x != y) != z) +> zs)
-
-lemma Bits.cons_carrySub_cons {n} (x y) (xs ys : Bits n) :
-  carrySub (x +> xs) (y +> ys) =
-    ((!x && (y != (carrySub xs ys).fst)) || (y && (carrySub xs ys).fst), ((x != y) != (carrySub xs ys).fst) +> (carrySub xs ys).snd) := rfl
-
--- def Bits.sub {n} : Bits n → Bits n → Bits n --:= (carrySub xs ys).snd
---   | ⦃⦄, ⦃⦄ => ⦃⦄
---   | x +> xs, y +> ys => ((x != y) != decide (xs < ys)) +> sub xs ys
-
-def Bits.sub {n} : Bits n → Bits n → Bits n --:= (carrySub xs ys).snd
+def Bits.sub {n} : Bits n → Bits n → Bits n
   | ⦃⦄, ⦃⦄ => ⦃⦄
   | x +> xs, y +> ys => ((x != y) != lt' xs ys) +> sub xs ys
 
@@ -482,7 +361,7 @@ lemma Bits.faux : ∀ {n} {xs ys : Bits n}, lt' xs ys = overflow (xs - ys) ys :=
 lemma Bits.lt_irrefl {n} {xs : Bits n} : ¬ xs < xs := by
   intro h;
   induction n with
-  | zero => cases xs; cases h  --simp [LT.lt, lt]
+  | zero => cases xs; cases h
   | succ n ih =>
     match xs with
     | x +> xs =>
@@ -498,138 +377,41 @@ lemma Bits.cons_sub_cons {n} {x y} {xs ys : Bits n} :
 lemma Bits.cons_add_cons {n} {x y} {xs ys : Bits n} :
     (x +> xs) + (y +> ys) = ((x != y) != overflow xs ys) +> (xs + ys) := rfl
 
--- #exit
--- lemma Bits.cons_sub_cons {n} {x y} {xs ys : Bits n} :
---     carrySub (x +> xs) (y +> ys) =
---       ⟨(!x && (y != (xs < ys))) || (y && (xs < ys)), ((x != y) != (xs < ys)) +> (xs - ys)⟩ := by
---   induction n generalizing x y with
---   | zero =>
---     cases xs; cases ys
---     simp [carrySub, Bool.zero, lt_irrefl]
---     apply nil_eq_nil
---   | succ n ih =>
---     match xs, ys with
---     | x' +> xs, y' +> ys =>
---       rw [cons_carrySub_cons x y, ih]
---       apply congr_arg₂
---       · apply congr_arg₂
---         · apply congr_arg₂
---           · rfl
---           · simp;
---
-
-
-
-
-
-
-
-
-
-
-
-
-
-
-
-
-
-
-
-
-
-
-
-
-
-
-
-
-
-
-
-
---     x +> xs - y +> ys = decr y ((xs - ys) +> x) := rfl
-
-
--- lemma Bits.cons_add_cons {n} {xs ys : Bits n} {x y} :
---     x +> xs + y +> ys = incr x ((xs + ys) +> y) := rfl
---
--- lemma Bits.cons_zero_add_cons {n} {xs ys : Bits n} {y} :
---     xs +> 0 + y +> ys = ((xs + ys) +> y) := rfl
---
--- lemma Bits.cons_add_cons_zero {n} {xs ys : Bits n} {x} :
---     x +> xs + ys +> 0 = ((xs + ys) +> x) := by
---   rw [cons_add_cons]; cases x <;> simp [incr] <;> rfl
---
--- lemma Bits.cons_add_cons_one {n} {xs ys : Bits n} {x} :
---     x +> xs + ys +> 1 = ((xs + ys) +> x).succ := by
---   rw [cons_add_cons]; cases x <;> simp [incr] <;> rfl
---
--- lemma Bits.cons_false_add_cons {n} {xs ys : Bits n} {y} :
---     xs +> false + y +> ys = ((xs + ys) +> y) := cons_zero_add_cons
---
--- lemma Bits.cons_true_add_cons {n} {xs ys : Bits n} {y} :
---     xs +> true + y +> ys = ((xs + ys) +> y).succ := rfl
---
--- lemma Bits.cons_add_cons_false {n} {xs ys : Bits n} {x} :
---     x +> xs + ys +> false = ((xs + ys) +> x) := cons_add_cons_zero
---
--- lemma Bits.cons_add_cons_true {n} {xs ys : Bits n} {x} :
---     x +> xs + ys +> true = ((xs + ys) +> x).succ := cons_add_cons_one
-
--- lemma Bits.cons_sub_cons_true {n} {xs ys : Bits n} {x} :
---     x +> xs - ys +> true = ((xs - ys) +> x).pred := rfl
---
--- lemma Bits.cons_sub_cons_false {n} {xs ys : Bits n} {x} :
---     x +> xs - ys +> false = (xs - ys) +> x := rfl
---
--- lemma Bits.cons_sub_cons {n} {xs ys : Bits n} {x y} :
---     x +> xs - y +> ys = decr y ((xs - ys) +> x) := rfl
---
--- lemma Bits.cons_sub_cons' {n} {xs ys : Bits n} {x} :
---     x +> xs - ys +> x = (xs - ys) +> 0 := by cases x <;> rfl
-
--- def Bits.carryShlo : ∀ {n}, Bits n → Bool → (Bool × Bits n)
---   | 0, ⦃⦄, y => (y, ⦃⦄)
---   | _ + 1, x +> xs, y =>
---     let (z, zs) := carryShlo xs y
---     (x, z +> zs)
-
 def Bits.snoc : ∀ {n}, Bits n → Bool → Bits (n + 1)
   | 0, ⦃⦄, y => ⦃y⦄
   | _ + 1, x +> xs, y => x +> (xs.snoc y)
 
 def Bits.shlo : ∀ {n}, Bits n → Bool → Bits n
   | 0, ⦃⦄, _ => ⦃⦄
-  | _ + 1, _ +> xs, y => xs.snoc y
-
--- def Bits.shlo : ∀ {n}, Bits n → Bool → (Bits n
---   | 0, ⦃⦄, _ => ⦃⦄
---   | _ + 1, x +> xs, y => shlo xs x +> y
-
--- def Bits.shl : Nat → ∀ {n}, Bits n → Bits n
---   | 0, _, xs => xs
---   | k + 1, _, xs => shl k <| shlo xs 0
+  | _ + 1, _ +> xs, y => Bits.snoc xs y
 
 def Bits.shl : Nat → ∀ {n}, Bits n → Bits n
   | 0, _, xs => xs
   | _, 0, ⦃⦄ => ⦃⦄
   | m + 1, _ + 1, _ +> xs => (shl m xs).snoc 0
 
---def Bits.shl : Nat → ∀ {n}, Bits n → Bits n
---  | 0, _, xs => xs
---  | k + 1, _, xs => shlo (shl k xs) 0
+-- def Bits.shro : ∀ {n}, Bool → Bits n → Bits n
+--   | 0, _, ⦃⦄ => ⦃⦄
+--   | n + 1, x, y +> ys =>  x +> shro y ys
 
+--def Bits.shr' : ∀ {k m n : Nat}, Bits m → Bits n
+--| 0, m, n, xs => _
+--
+--#exit
+def Bits.prefixLe : ∀ {m n}, m ≤ n → Bits n → Bits m
+| 0, _, _, _ => ⦃⦄
+| m + 1, 0, h, _ => (Nat.not_succ_le_zero m h).elim
+| _ + 1, _ + 1, h, x +> xs =>
+  x +> prefixLe (Nat.le_of_succ_le_succ h) xs
 
-def Bits.shro : ∀ {n}, Bool → Bits n → Bits n
-  | 0, _, ⦃⦄ => ⦃⦄
-  | n + 1, x, y +> ys =>  x +> shro y ys
+def Bits.shr' : Nat → ∀ {m n}, m ≤ n → Bits n → Bits m
+  | _, 0, _, _, _ => ⦃⦄
+  | 0, _, _, h, xs => prefixLe h xs
+  | k + 1, m + 1, n, h, xs =>
+    0 +> @shr' k m n (le_trans (Nat.le_succ _) h) xs
 
-def Bits.shr : Nat → ∀ {n}, Bits n → Bits n
-  | 0, _, xs => xs
-  | k + 1, _, xs => --shro 0 (shr k xs)
-    shr k (shro 0 xs)
+def Bits.shr (m : Nat) {n} (xs : Bits n) : Bits n :=
+  Bits.shr' m (le_refl n) xs
 
 def Bits.isNeg : ∀ {n : ℕ}, Bits n → Bool
   | 0, _ => false
@@ -647,8 +429,6 @@ def Bits.append : ∀ {m n}, Bits m → Bits n → Bits (n + m)
   | m + 1, n, x +> xs, ys => x +> append xs ys
 
 instance {m n} : HAppend (Bits m) (Bits n) (Bits (n + m)) := ⟨Bits.append⟩
-
---lemma Bits.append_nil {n} {xs : Bits n} : xs ++ ⦃⦄ = xs :=  rfl
 
 lemma Bits.cons_append {m n} {x} {xs : Bits m} {ys : Bits n} :
     (x +> xs) ++ ys = x +> (xs ++ ys) := by rfl
@@ -675,7 +455,7 @@ instance {n} : HMul (Bits n) (Bits n) (Bits n) := ⟨Bits.mul⟩
 def divMod : ∀ {m n : ℕ}, Bits n → Bits m → Bits n → (Bits m × Bits n)
   | 0, _, pfx, ⦃⦄, _ => (0, pfx)
   | _ + 1, _, pfx, x +> xs, ys =>
-    let pfx' := .shlo pfx x
+    let pfx' := Bits.shlo pfx x
     if ys ≤ pfx'
     then let (div, mod) := divMod (pfx' - ys) xs ys
          (1 +> div, mod)
@@ -724,11 +504,6 @@ def Bits.addmod {n : ℕ} (x y z : Bits n) : Bits n :=
 def Bits.mulmod {n : ℕ} (x y z : Bits n) : Bits n :=
   if z = 0 then 0 else (x * y) % z
 
--- def Bits.iter {α : Type} (f : α → α) : α → ∀ {n}, Bits n → α
---   | a, 0, ⦃⦄ => a
---   | a, _ + 1, xs +> 0 => iter f (iter f a xs) xs
---   | a, _ + 1, xs +> 1 => iter f (iter f (f a) xs) xs
-
 def Bits.expNat {n : ℕ} (x : Bits n) : Nat → Bits n
   | 0 => 1
   | k + 1 => x * x.expNat k
@@ -746,11 +521,6 @@ inductive Bits.Signext' : Nat → Bool → ∀ {n}, Bits n → Bits n → Prop
 
 def Bits.Signext (x y y' : Word) : Prop :=
   ∃ b, Signext' (256 - (8 * (x.toNat + 1))) b y y'
-
--- def Bits.suffix : ∀ {m n}, Bits m → Bits n → Prop
---   | _, 0, _, ⦃⦄ => true
---   | 0, _ + 1, ⦃⦄, _ => false
---   | _ + 1, _ + 1, x +> xs, y +> ys => suffix xs ys ∧ x = y
 
 def Bits.prefix {m} : ∀ {n}, Bits (m + n) → Bits n
   | 0, _ => ⦃⦄
@@ -798,16 +568,6 @@ def Nat.toBits (k) : Nat → Bits k
 
 lemma Bits.zero_eq_cons {n} : (0 : Bits (n + 1)) = 0 +> (0 : Bits n) := rfl
 lemma Bits.max_eq_cons {n} : max (n + 1) = 1 +> max n := rfl
-lemma Bits.one_eq_cons {n} : (1 : Bits (n + 2)) = 0 +> (1 : Bits (n + 1)) := rfl
-
-lemma overflow_zero {n : ℕ} (xs : Bits n) : overflow xs 0 = false := by
-  induction n with
-  | zero => cases xs; rfl
-  | succ n ih =>
-    match xs with
-    | x +> xs =>
-      simp [Bits.zero_eq_cons, overflow, Bool.zero]
-      intro _; apply ih
 
 lemma Bits.eq_max_iff_isMax {k : ℕ} (xs : Bits k) : xs = max k ↔ xs.isMax = true := by
   induction xs with
@@ -819,15 +579,6 @@ lemma Bits.eq_max_iff_isMax {k : ℕ} (xs : Bits k) : xs = max k ↔ xs.isMax = 
 lemma Bits.max_isMax {n : ℕ} : (max n).isMax = true := by
   rw [← eq_max_iff_isMax]
 
-lemma Bits.eq_max_iff_succ_eq_zero {k : ℕ} (xs : Bits k) :
-    xs = max k ↔ xs.succ = 0 := by
-  induction xs with
-  | nil => apply iff_of_true <;> rfl
-  | cons x xs ih =>
-    rw [succ, zero_eq_cons, max_eq_cons, cons_eq_cons, cons_eq_cons, ih]
-    simp; intro h; rw [← ih, eq_max_iff_isMax] at h
-    rw [h]; cases x <;> simp [Bool.one, Bool.zero]
-
 lemma Bits.succ_toNat_max_eq_pow {n : Nat} : (max n).toNat.succ = 2 ^ n := by
   induction n with
   | zero => rfl
@@ -835,7 +586,6 @@ lemma Bits.succ_toNat_max_eq_pow {n : Nat} : (max n).toNat.succ = 2 ^ n := by
 
 lemma Bits.toNat_max_add_one_eq_pow {n : Nat} : (max n).toNat + 1 = 2 ^ n :=
   succ_toNat_max_eq_pow
-
 
 lemma Bits.toNat_succ {k : ℕ} (xs : Bits k) :
     xs.succ.toNat = cond xs.isMax 0 xs.toNat.succ := by
@@ -850,37 +600,6 @@ lemma Bits.toNat_succ {k : ℕ} (xs : Bits k) :
       simp [h'] at ih
       simp only [succ, toNat, isMax, h']
       rw [← Nat.add_succ]; simp [ih]
-
--- lemma Nat.toBits_inj {k m n : ℕ} (hm : m < 2 ^ k) (hn : n < 2 ^ k)
---     (h : toBits k m = toBits k n) : m = n := by
---   -- | 0, m, n, hm, hn, h => by
---   --   match m, n with
---   --   | succ _, _ =>
---   have foo : ∀ {k m : Nat}, m + 1 < 2 ^ k → (toBits k 0) ≠ (toBits k (m + 1)) := by
---     clear hm hn h k m n
---     intro k m h h'
---     simp only [toBits] at h'
---     rw [Eq.comm, ← Bits.eq_max_iff_succ_eq_zero] at h'
---
---   induction m generalizing n with
---   | zero =>
---     match n with
---     | 0 => rfl
---     | n + 1 =>
---       simp [toBits] at h
---   | succ m ih =>
---     match n with
---     | 0 =>
---     | n + 1 =>
---       have hm' := lt_trans (Nat.lt_succ_self m) hm
---       have hn' := lt_trans (Nat.lt_succ_self n) hn
---       rw [ih hm' hn' <| Bits.succ_inj h]
-
-
-
-
-
-
 
 instance {m n} : OfNat (Bits m) n := ⟨Nat.toBits _ n⟩
 
@@ -911,27 +630,13 @@ def Bits.toBytes : ∀ {n}, Bits (8 * n) → Bytes
   | _ + 1, b0 +> b1 +> b2 +> b3 +> b4 +> b5 +> b6 +> b7 +> bs =>
     ⦃b0, b1, b2, b3, b4, b5, b6, b7⦄ :: bs.toBytes
 
-def Bits.min {n} (x y : Bits n) : Bits n := if x ≤ y then x else y
-
--- #check List.takeD
--- def Bytes.ekatD' : Nat → Bytes → Byte → (Nat × Bytes)
---   | k, [], _ => (k, [])
---   | k, b :: bs, c =>
---     match ekatD' k bs c with
---     | (0, bs') => (0, bs')
---     | (k' + 1, bs') => (k', b :: bs')
---
 def Bytes.toBits' : ∀ (n : Nat), Bytes → Bits (8 * n)
   | 0, _ => ⦃⦄
   | n + 1, [] => (0 : Byte) ++ toBits' n []
   | n + 1, b :: bs => b ++ toBits' n bs
 
 def Bytes.toBits (n : Nat) (bs : Bytes) : Bits (8 * n) :=
-  --have h : bs'.length = n := by
-  --  rw [List.length_reverse]; apply List.takeD_length
-  --by rw [← h]; exact
   Bytes.toBits' n <| List.reverse <| List.takeD n (List.reverse bs) 0
-
 
 lemma Bits.cons_eq_zero_iff {n x} {xs : Bits n} :
    x +> xs = 0 ↔ (x = 0 ∧ xs = 0) := by rw [zero_eq_cons]; simp
@@ -945,189 +650,13 @@ lemma Bits.zero_append_zero {m n} :
 lemma Bits.toNat_zero : ∀ {k}, (0 : Bits k).toNat = 0
   | 0 => rfl
   | k + 1 => by rw [zero_eq_cons]; simp [toNat, @toNat_zero k]; rfl
---
---
--- lemma Bits.of_toNat_eq_zero {k} (xs : Bits k) (h : xs.toNat = 0) : xs = 0 := by
---   induction k with
---   | zero => apply nil_eq_nil
---   | succ k ih =>
---     rcases xs with _ | ⟨xs, _ | _⟩ <;>
---     (simp [cons_eq_zero_iff]; simp [toNat, Nat.mul_eq_zero] at h)
---     · refine ⟨ih _ h, false_eq_zero⟩
---
--- lemma Bits.nonzero_toNat {k} (xs : Bits k) : xs ≠ 0 → xs.toNat ≠ 0 :=
---   mt <| of_toNat_eq_zero xs
---
--- lemma Bits.succ_toNat_assoc {k} : (xs : Bits k) → xs ≠ max _ → xs.succ.toNat = xs.toNat.succ := by
---   apply @Nat.rec (λ k => (xs : Bits k) → xs ≠ max _ → xs.succ.toNat = xs.toNat.succ)
---   · intros xs h; cases h nil_eq_nil
---   · intros k ih xs h; rcases xs with _ | ⟨xs, _ | _⟩
---     · simp [succ, toNat, false_toNat, true_toNat, Bool.zero_toNat, Bool.one_toNat]
---     · simp [succ, toNat, false_toNat, true_toNat, Bool.zero_toNat, Bool.one_toNat]
---       have h_ne : xs ≠ max _ := by
---         intro hc; simp [max, hc] at h
---       rw [ih _ h_ne]; simp [Nat.mul_succ]
---
--- lemma Bits.incr_toNat_assoc {k} (x) (xs : Bits k) (h : xs ≠ max _) :
---     (incr x xs).toNat = xs.toNat + x.toNat := by
---   cases x <;> simp [incr]; apply succ_toNat_assoc _ h
---
-lemma Bits.nil_toNat (xs : Bits 0) : xs.toNat = 0 := by cases xs; rfl
---
--- lemma Bits.pred_toNat_assoc {k} (xs : Bits k) (h : xs ≠ 0) : xs.pred.toNat = xs.toNat.pred := by
---   induction k with
---   | zero => simp [nil_toNat]
---   | succ k ih =>
---     rcases xs with _ | ⟨xs, _ | _⟩ <;>
---     simp [pred, toNat, Bool.one_toNat]
---     · simp [Ne, cons_eq_zero_iff, false_eq_zero] at h; rw [ih xs h];
---       rcases Nat.exists_eq_succ_of_ne_zero <| nonzero_toNat _ h with ⟨n, hn⟩
---       rw [hn, Nat.mul_succ]; simp [Nat.pred]
---     · rfl
---
--- lemma Bits.decr_toNat_assoc {k} (x) (xs : Bits k) (h : xs ≠ 0) :
---     (decr x xs).toNat = xs.toNat - x.toNat := by
---   cases x <;> simp [decr]; apply pred_toNat_assoc _ h
---
 
--- lemma Bits.succ_pred : ∀ {n} {xs : Bits n}, succ (pred xs) = xs := by
---   apply Nat.rec
---   · intros _; apply nil_eq_nil
---   · intros n ih xs; rcases xs with _ | ⟨xs, _ | _⟩ <;> simp [pred, succ]
---     · simp [ih]; rfl
---     · rfl
---
--- lemma Bits.pred_succ : ∀ {n} {xs : Bits n}, pred (succ xs) = xs := by
---   apply Nat.rec
---   · intros _; apply nil_eq_nil
---   · intros n ih xs; rcases xs with _ | ⟨xs, _ | _⟩ <;> simp [pred, succ]
---     · rfl
---     · simp [ih]; rfl
---
--- lemma Bits.add_comm : ∀ {n} {xs ys : Bits n}, xs + ys = ys + xs := by
---   apply Nat.rec
---   · intros _ _; apply nil_eq_nil
---   · intros n ih xs ys;
---     rcases xs with _ | ⟨xs, x⟩
---     rcases ys with _ | ⟨ys, y⟩
---     rw [cons_add_cons, cons_add_cons, ih];
---     cases x <;> cases y <;> rfl
---
--- lemma Bits.succ_add : ∀ {n} {xs ys : Bits n}, succ (xs + ys) = xs.succ + ys := by
---   apply Nat.rec
---   · intros _ _; apply nil_eq_nil
---   · intros n ih xs ys;
---     rcases xs with _ | ⟨xs, _ | _⟩ <;>
---     rcases ys with _ | ⟨ys, _ | _⟩
---     · rfl
---     · rfl
---     · rw [cons_add_cons_false]; simp [succ];
---       rw [cons_add_cons_false, ih]
---     · rw [cons_true_add_cons]; simp [succ];
---       rw [cons_add_cons_true]; simp [succ, ih]
---
--- lemma Bits.pred_add_eq_add_pred : ∀ {n} {xs ys : Bits n}, xs.pred + ys = xs + ys.pred := by
---   apply Nat.rec
---   · intros _ _; apply nil_eq_nil
---   · intros n ih xs ys;
---     rcases xs with _ | ⟨xs, _ | _⟩ <;>
---     rcases ys with _ | ⟨ys, _ | _⟩
---     · simp [cons_false_add_cons, pred, cons_add_cons_false]; apply ih
---     · simp [pred, cons_add_cons, incr, succ];
---       rw [succ_add]; simp [succ_pred]
---     · simp [pred]; rw [cons_add_cons_false, cons_true_add_cons];
---       simp [succ]; rw [← ih, succ_add, succ_pred];
---     · rfl
---
--- lemma Bits.pred_add : ∀ {n} {xs ys : Bits n}, pred (xs + ys) = xs.pred + ys := by
---   apply Nat.rec
---   · intros _ _; apply nil_eq_nil
---   · intros n ih xs ys;
---     rcases xs with _ | ⟨xs, _ | _⟩ <;>
---     rcases ys with _ | ⟨ys, _ | _⟩
---     · simp [cons_false_add_cons, pred, cons_add_cons_false]; apply ih
---     · rw [cons_false_add_cons, pred_add_eq_add_pred]
---       simp [pred]; rfl
---     · rfl
---     · rw [cons_true_add_cons]; simp [pred];
---       rw [cons_add_cons_true]; simp [succ, pred_succ]
---
--- lemma Bits.pred_sub : ∀ {n} {xs ys : Bits n}, pred (xs - ys) = xs.pred - ys := by
---   apply Nat.rec
---   · intros _ _; apply nil_eq_nil
---   · intros n ih xs ys;
---     rcases xs with _ | ⟨xs, _ | _⟩ <;>
---     rcases ys with _ | ⟨ys, _ | _⟩
---     · rw [cons_sub_cons_false]; simp [pred]; rw [cons_sub_cons_false, ih]
---     · rw [cons_sub_cons_true]; simp [pred]; rw [cons_sub_cons_true]; simp [pred, ih]
---     · rfl
---     · rfl
---
--- lemma Bits.succ_sub : ∀ {n} {xs ys : Bits n}, succ (xs - ys) = xs.succ - ys := by
---   apply Nat.rec
---   · intros _ _; apply nil_eq_nil
---   · intros n ih xs ys;
---     rcases xs with _ | ⟨xs, _ | _⟩ <;>
---     rcases ys with _ | ⟨ys, _ | _⟩
---     · rw [cons_sub_cons_false]; simp [succ]; rw [cons_sub_cons_false]
---     · simp [succ]; rw [succ_pred]; rfl
---     · rw [cons_sub_cons_false]; simp [succ]; rw [cons_sub_cons_false, ih]
---     · simp [succ]; rw [cons_sub_cons_true]; simp [pred];
---       rw [pred_sub, pred_succ]; rfl
---
--- lemma Bits.pred_add' {n} {xs ys : Bits n} : pred (xs + ys) = xs + ys.pred := by
---   rw [@add_comm _ _ ys, pred_add, add_comm]
---
--- lemma Bits.add_sub_assoc : ∀ {n} {xs ys zs : Bits n}, xs + ys - zs = xs + (ys - zs) := by
---   apply Nat.rec
---   · intros _ _ _; apply nil_eq_nil
---   · intros m ih xs ys zs
---     rcases xs with _ | ⟨xs, _ | _⟩ <;>
---     rcases ys with _ | ⟨ys, _ | _⟩ <;>
---     rcases zs with _ | ⟨zs, _ | _⟩ <;>
---     simp [cons_add_cons, cons_sub_cons, decr, incr]
---     · rw [ih]
---     · rw [← pred_add', cons_false_add_cons, ih]
---     · rw [ih]
---     · rw [← pred_add', cons_false_add_cons, ih]
---     · simp [succ]; rw [cons_sub_cons_false, ih]
---     · simp [succ]; rw [← pred_add_eq_add_pred];
---       simp [pred]; rw [cons_zero_add_cons, ← ih]; rfl
---     · simp [succ]; rw [cons_sub_cons_false];
---       rw [← ih, succ_sub]
---     · simp [succ, pred]; rw [cons_sub_cons_true, cons_true_add_cons]
---       simp [succ, pred]; rw [pred_sub, pred_succ, ih]
-
-
- -- apply Nat.rec
- -- · intros _; apply nil_eq_nil
- -- · intros m ih xs; rcases xs with _ | ⟨xs, x⟩
- --   rw [cons_sub_cons', ih]; rfl
---
--- lemma Bits.add_sub_cancel {n} {x y : Bits n} : x + y - y = x :=
---  by rw [add_sub_assoc, sub_self, add_zero]
---
--- lemma Bits.add_sub_comm {n} {xs ys zs : Bits n} : xs + ys - zs = xs - zs + ys := by
---   rw [add_comm, add_sub_assoc, add_comm]
---
 lemma Bits.sub_add_cancel : ∀ {n} {x y : Bits n}, x - y + y = x := by
   apply rec2; rfl
   intro n x xs y ys ih
   rw [cons_sub_cons, cons_add_cons, ih]
   apply congr_arg₂ _ _ rfl
   rw [← Bits.faux]; cases (lt' xs ys) <;> cases y <;> simp
-
---by rw [← add_sub_comm, add_sub_cancel]
-
---
--- lemma Bits.zero_add {n} (xs : Bits n) : 0 + xs = xs := by rw [add_comm, add_zero]
---
--- lemma Bits.add_right_inj {n} {x y z : Bits n} : x + z = y + z → x = y := by
---   intro h; have h' : x + z - z = y + z - z := by rw [h]
---   rw [add_sub_assoc, add_sub_assoc, sub_self, add_zero, add_zero] at h'; exact h'
---
--- lemma Bits.add_left_inj {n} {x y z : Bits n} : z + x = z + y → x = y := by
---  rw [add_comm, @add_comm _ z]; apply add_right_inj
 
 lemma Bits.add_left_inj {n} :
     ∀ {xs ys zs : Bits n}, xs + ys = xs + zs → ys = zs := by
@@ -1165,7 +694,6 @@ lemma Bits.eq_max_iff_succ_toNat_eq_pow {n : Nat} (xs : Bits n) :
   · rw [h]; apply succ_toNat_max_eq_pow
   · apply toNat_inj; rw [← Nat.succ_inj, succ_toNat_max_eq_pow, h]
 
-
 lemma toNat_toBits {k n} (h : n < 2 ^ k) : (Nat.toBits k n).toNat = n := by
   induction n with
   | zero => simp [Nat.toBits, Bits.toNat, Bits.toNat_zero]
@@ -1182,27 +710,6 @@ lemma Nat.toBits_inj {k m n : ℕ} (hm : m < 2 ^ k) (hn : n < 2 ^ k)
     (h : toBits k m = toBits k n) : m = n := by
   rw [← toNat_toBits hm, ← toNat_toBits hn, h]
 
-
-
-
-
-
-
-
-
-
-
--- lemma toBits_toNat {k} : ∀ n, n < 2 ^ k → (@Nat.toBits k n).toNat = n := by
---   apply Nat.rec
---   · simp [Nat.toBits, Bits.toNat, Bits.zero_toNat]
---   · intros n ih h_lt
---     have h_lt' : n < 2 ^ k := Nat.lt_trans (Nat.lt_succ_self _) h_lt
---     have ih' := ih h_lt'
---     unfold Nat.toBits; rw [Bits.succ_toNat_assoc, ih']
---     intro hc; rw [hc] at ih'
---     rw [← ih', Bits.max_toNat_succ] at h_lt
---     apply Nat.lt_irrefl _ h_lt
---
 lemma Bits.nil_le_nil {xs ys : Bits 0} : xs ≤ ys := by
   cases xs; cases ys; constructor
 
@@ -1238,10 +745,6 @@ lemma Bits.le_refl {n} {xs : Bits n} : xs ≤ xs := by
   | nil => apply nil_le_nil
   | cons x xs ih => simp [cons_le_cons]; exact ih
 
--- lemma Bits.le_of_eq {n : Nat} {xs ys : Bits n} (h : xs = ys) : xs ≤ ys := by
---   cases h; apply le_refl
---
-
 lemma Bits.le_of_lt {n : Nat} {xs ys : Bits n} (h : xs < ys) : xs ≤ ys := by
   induction n with
   | zero => cases xs; cases ys; cases h
@@ -1252,11 +755,6 @@ lemma Bits.le_of_lt {n : Nat} {xs ys : Bits n} (h : xs < ys) : xs ≤ ys := by
       rcases h with h | ⟨h, h'⟩
       · left; exact h
       · right; refine ⟨h, ih h'⟩
-
-
--- lemma Bits.le_of_lt_or_eq {n : Nat} {xs ys : Bits n}
---     (h : xs < ys ∨ xs = ys) : xs ≤ ys := by
---   cases h; apply le_of_lt asm; apply le_of_eq asm
 
 lemma Bits.lt_or_eq_of_le {n : Nat} {xs ys : Bits n} (h : xs ≤ ys) :
     xs < ys ∨ xs = ys := by
@@ -1270,43 +768,6 @@ lemma Bits.lt_or_eq_of_le {n : Nat} {xs ys : Bits n} (h : xs ≤ ys) :
       · rcases ih h with h | ⟨⟨_⟩⟩
         · left; right; refine ⟨rfl, h⟩
         · right; rfl
-
--- lemma Bits.lt_or_eq_of_le {n : Nat} {xs ys : Bits n} (h : xs ≤ ys) : xs < ys ∨ xs = ys := by
---   cases n with
---   | zero => right; apply nil_eq_nil
---   | succ n  =>
---   match xs, ys with
---   | x +> xs, y +> ys =>
---     cases h with
---     | inl h' => left; left; apply h'
---     | inr h' =>
---       match x, y with
---       | 0, 0 => right; rw [h'.left]
---       | 0, 1 => left; right; simp [h'.left]; constructor
---       | 1, 0 => simp [LE.le] at h'
---       | 1, 1 => right; rw [h'.left]
---
---
--- lemma Bits.le_iff_lt_or_eq {n : Nat} {xs ys : Bits n} : xs ≤ ys ↔ (xs < ys ∨ xs = ys) :=
---   ⟨lt_or_eq_of_le, le_of_lt_or_eq⟩
---
--- lemma Bits.cons_lt_cons_of_le_of_lt {n} {xs ys : Bits n} {x y} :
---     xs ≤ ys → x < y → x +> xs < y +> ys := by
---   intros hs h; cases lt_or_eq_of_le hs with
---   | inl h_lt => left; apply h_lt
---   | inr h_eq => right; refine ⟨h_eq, h⟩
---
--- lemma Bits.le_max {n} : ∀ {xs : Bits n}, xs ≤ max _ := by
---   induction n with
---   | zero => intro _; apply nil_le_nil
---   | succ n ih =>
---     intro xs
---     cases xs with
---     | cons xs x =>
---       cases lt_or_eq_of_le ih with
---       | inl h => left; apply h
---       | inr h => right; refine' ⟨h, Bool.le_one⟩
---
 
 lemma Bits.zero_le {n} : ∀ xs : Bits n, 0 ≤ xs := by
   induction n with
@@ -1329,38 +790,6 @@ lemma Bits.le_of_le_of_lt {n} {xs ys zs : Bits n}
     (h : xs ≤ ys) (h' : ys < zs) : xs ≤ zs :=
   le_of_lt <| lt_of_le_of_lt h h'
 
-lemma Bits.lt_of_lt_of_le {n} {xs ys zs : Bits n}
-    (h : xs < ys) (h' : ys ≤ zs) : xs < zs := by
-  cases lt_or_eq_of_le h' with
-  | inl h'' => apply lt_trans h h''
-  | inr h'' => rw [← h'']; exact h
-
--- lemma Bits.le_trans {n} {xs ys zs : Bits n} (h : xs ≤ ys) (h' : ys ≤ zs) : xs ≤ zs := by
---   induction n with
---   | zero => cases xs; cases zs; constructor
---   | succ n ih =>
---     match xs, ys, zs with
---     | x +> xs, y +> ys, zs +> z =>
---       cases x <;> cases y <;> cases z <;>
---       simp [cons_le_cons, false_le, not_true_le_false] at * <;>
---       try {apply lt_or_eq_of_le (ih (le_of_lt_or_eq h) (le_of_lt_or_eq h'))}
---       · left; apply lt_of_le_of_lt (le_of_lt_or_eq h) h'
---       · apply lt_of_lt_of_le h <| le_of_lt_or_eq h'
---       · apply lt_or_eq_of_le <| ih (le_of_lt h) <| le_of_lt_or_eq h'
---       · apply lt_of_le_of_lt (le_of_lt_or_eq h) h'
---
--- lemma Bits.lt_max_of_ne_max {n} {xs : Bits n} : xs ≠ max _ → xs < max _ := by
---   induction n with
---   | zero => intro h; cases h nil_eq_nil
---   | succ n ih =>
---     rcases xs with _ | ⟨xs, _ | _⟩ <;> unfold max
---     · simp; apply cons_lt_cons_of_le_of_lt le_max cst
---     · rw [true_eq_one]; simp; intro h; left; apply ih h
---
--- lemma Bits.lt_max_iff_ne_max {n} {xs : Bits n} : xs < max _ ↔ xs ≠ max _ := by
---   refine' ⟨λ h_lt h_eq => _, lt_max_of_ne_max⟩
---   cases h_eq; apply lt_irrefl h_lt
-
 lemma Nat.toBits_le_toBits {k m n : Nat} (h_le : m ≤ n) (h_lt : n < 2 ^ k) :
     (@toBits k m) ≤ (@toBits k n) := by
   induction n generalizing m with
@@ -1377,28 +806,6 @@ lemma Nat.toBits_le_toBits {k m n : Nat} (h_le : m ≤ n) (h_lt : n < 2 ^ k) :
       rw [Bits.eq_max_iff_succ_toNat_eq_pow, toNat_toBits h_lt'] at hc
       rw [← hc] at h_lt; cases Nat.lt_irrefl _ h_lt
     · rw [h_eq]; apply Bits.le_refl
-
--- lemma toBits_le_toBits {k m n : Nat} :
---      m ≤ n → n < 2 ^ k → (@Nat.toBits k m) ≤ (@Nat.toBits k n) := by
---   revert m
---   induction n with
---   | zero => intros m h_le h_lt; cases m; apply Bits.zero_le; cases h_le
---   | succ n ih =>
---     intros m h_le h_lt;
---     cases Nat.lt_or_eq_of_le h_le with
---     | inl h_lt' =>
---       apply
---         Bits.le_trans
---           (ih (Nat.le_of_lt_succ h_lt') (Nat.lt_trans (Nat.lt_succ_self _) h_lt))
---       apply Bits.le_of_lt; apply Bits.lt_succ_self
---       rw [Bits.lt_max_iff_ne_max]; intro h_eq
---       have h_eq' : n + 1 = 2 ^ k := by
---         apply Eq.trans _ Bits.max_toNat_succ; simp
---         rw [← h_eq, toBits_toNat]
---         apply Nat.lt_trans _ h_lt; simp
---       rw [h_eq'] at h_lt; apply Nat.lt_irrefl _ h_lt
---     | inr h_eq => rw [← h_eq]; apply Bits.le_refl
---
 
 abbrev Hex : Type := Bits 4
 
@@ -1429,16 +836,10 @@ def Byte.hex1 : Byte → Hex
 def Byte.toString (b : Byte) : String :=
 ⟨[Hex.toChar b.hex0, Hex.toChar b.hex1]⟩
 
-def Byte.toString' (b : Byte) : String :=
-⟨[b.hex0.toChar, b.hex1.toChar]⟩
-
 def Bytes.toString : Bytes → String
   | [] => ""
   | [b] => b.toString
   | b :: bs => b.toString ++ " " ++ toString bs
-
-def Bytes.toString' (bs : Bytes) : String :=
-  "0x" ++ List.foldr (λ b s => b.toString ++ s) "" bs
 
 instance : Repr Bytes := ⟨λ b _ => b.toString⟩
 
@@ -1464,10 +865,6 @@ def xD : Hex := ⦃1, 1, 0, 1⦄
 def xE : Hex := ⦃1, 1, 1, 0⦄
 def xF : Hex := ⦃1, 1, 1, 1⦄
 
---def Bytes.length : Bytes → Nat
---  | [] => 0
---  | bs :> _ => bs.length + 1
-
 lemma List.length_dropWhile_le {ξ : Type u} (xs : List ξ) (f : ξ → Bool) :
     (dropWhile f xs ).length ≤ xs.length := by
   induction xs with
@@ -1480,43 +877,6 @@ lemma List.length_dropWhile_le {ξ : Type u} (xs : List ξ) (f : ξ → Bool) :
 
 def Bytes.sig (bs : Bytes) : Bytes :=
   List.dropWhile (· = 0) bs
-
--- def Bytes.sig : Bytes → Bytes
---   | [] => []
---   | bs :> b =>
---   match bs.sig with
---   | [] => if b = 0 then [] else [b]
---   | bs'@(_ :> _) => bs' :> b
---
--- lemma Bytes.sig_length_le (bs : Bytes) : bs.sig.length ≤ bs.length := by
---   induction bs with
---   | nil => simp [Bytes.length]
---   | cons bs b ih =>
---     unfold Bytes.sig; revert ih
---     cases bs.sig with
---     | nil =>
---       simp; intro _
---       apply ite_cases (λ bs' : Bytes => bs'.length ≤ (bs :> b).length) <;>
---       intro _ <;> simp [Bytes.length]
---     | cons bs' b' =>
---       simp; intro h; simp [Bytes.length]; apply h
-
--- lemma eq_nil_or_eq_cons (bs : Bytes) : bs = [] ∨ ∃ bs' b, bs = (bs' :> b) := by
---   cases bs; left; rfl; right; refine ⟨_, _, rfl⟩
-
--- lemma Bits.cons_eq_max {n} (xs : Bits n) (x) :
---     x +> xs = max _ ↔ (xs = max _ ∧ x = 1) := by
---   cases x
---   · apply iff_of_false <;> intro h
---     · cases h
---     · cases h.right
---   · cases em (xs = max _) with
---     | inl h => rw [h]; apply iff_of_true; rfl; simp; rfl
---     | inr h =>
---       apply iff_of_false <;> intro h'
---       · cases h'; cases h rfl
---       · cases h h'.left
---
 
 lemma Bool.lt_or_ge (x y : Bool) : x < y ∨ x ≥ y := by
   cases x <;> cases y <;> simp
@@ -1541,33 +901,10 @@ lemma Bits.lt_or_ge {n : ℕ} : ∀ xs ys : Bits n, xs < ys ∨ xs ≥ ys := by
           · left; right; refine ⟨h'.symm, h''⟩
           · right; right; refine ⟨h', h''⟩
 
--- lemma Bits.lt_or_ge {n : ℕ} : ∀ xs ys : Bits n, xs < ys ∨ xs ≥ ys := by
---   induction n with
---   | zero => intros _ _; right; apply nil_le_nil
---   | succ n ih =>
---     intros xs ys
---     match xs, ys with
---     | x +> xs, y +> ys =>
---       rcases ih xs ys with h | h
---       · left; left; exact h
---       · simp only [GE.ge] at h
---         rw [le_iff_lt_or_eq] at h
---         rcases h with h | h
---         · right; left; exact h
---         · rw [h]; cases x
---           · cases y
---             · right; right; simp
---             · left; right; simp; constructor
---           · right; right; simp
-
 lemma Bits.not_lt {n : ℕ} (xs ys : Bits n) : ¬ xs < ys ↔ ys ≤ xs := by
   constructor
   · rw [← or_iff_not_imp_left]; apply lt_or_ge
   · intros h h'; cases lt_irrefl <| lt_of_le_of_lt h h'
-
-lemma Bits.exists_eq_cons {n} (xs : Bits (n + 1)) : ∃ xs' x, xs = xs' +> x :=
-  by cases xs; refine ⟨_, _, rfl⟩
-
 
 lemma overflow_iff_overflow_eq_true :
     ∀ {n : ℕ} (xs ys : Bits n), Overflow xs ys ↔ overflow xs ys = true := by
@@ -1586,57 +923,6 @@ lemma overflow_iff_overflow_eq_true :
       simp [Overflow]
     · omega
 
-
-
-
-
-
-
-
-
-
-
-
-
--- lemma Bits.toNat_lt_toNat {k} (xs ys : Bits k) (h : xs < ys) : xs.toNat < ys.toNat := by
---   induction k with
---   | zero => cases xs; cases ys; cases h
---   | succ k ih =>
---     match xs, ys with
---     | x +> xs, y +> ys =>
---       rw [cons_lt_cons] at h
---       rcases h with h | ⟨h_eq, h_lt⟩
---       · simp [toNat]
---         apply @Nat.lt_of_lt_of_le _ (2 * xs.toNat + 2 * 1)
---         · apply Nat.add_lt_add_left; cases x <;> simp [Bool.toNat]
---         · rw [← Nat.mul_add]
---           apply @Nat.le_trans _ (2 * ys.toNat)
---           · apply Nat.mul_le_mul_left _ <| Nat.succ_le_of_lt <| ih _ _ h
---           · apply Nat.le_add_right
---       · cases x <;> cases y <;>
---         try {simp [LT.lt] at h_lt; done}
---         simp [h_eq, toNat]
---
--- lemma Bits.lt_succ_of_le  {k} {xs ys : Bits k}
---     (h : ys ≠ max k) (h' : xs ≤ ys) : xs < ys.succ := by
---   induction k with
---   | zero => cases h nil_eq_nil
---   | succ k ih =>
---     match xs, ys with
---     | x +> xs, y +> ys =>
---       rw [cons_le_cons] at h'
---       simp [Ne, cons_eq_max] at h; cases y
---       · simp [succ]; rcases h' with h' | h'
---         · rw [cons_lt_cons]; left; apply h'
---         · rw [cons_lt_cons, Bool.eq_false_of_le_false h'.right]
---           right; refine ⟨h'.left, cst⟩
---       · simp [true_eq_one] at h; simp [succ]
---         rw [cons_lt_cons]; left; apply ih h
---         apply le_of_lt_or_eq; rcases h' with h' | h'
---         · left; exact h'
---         · right; exact h'.left
---
-
 lemma Bits.toNat_lt_toNat :
     ∀ {k} (xs ys : Bits k), xs < ys → xs.toNat < ys.toNat := by
   apply rec2
@@ -1652,84 +938,6 @@ lemma Bits.toNat_le_toNat {k} (xs ys : Bits k) (h : xs ≤ ys) :
   rcases lt_or_eq_of_le h with h | ⟨⟨_⟩⟩
   · apply Nat.le_of_lt <| toNat_lt_toNat _ _ h
   · apply Nat.le_refl
-
--- lemma Bits.toNat_le_toNat {k} (xs ys : Bits k) (h : xs ≤ ys) : xs.toNat ≤ ys.toNat := by
---   by_cases h' : ys = max k
---   · apply Nat.le_of_lt_succ; rw [h', max_toNat_succ]; apply toNat_lt_pow
---   · apply Nat.le_of_lt_succ; rw [← succ_toNat_assoc _ h']
---     apply toNat_lt_toNat _ _ <| lt_succ_of_le h' h
---
--- lemma Bits.nof_of_add_eq_max {k} (xs ys : Bits k) (h : xs + ys = max _) :
---     Nof xs ys := by
---   induction k with
---   | zero => cases xs; cases ys; simp [Nof]; rfl
---   | succ k ih =>
---     match xs, ys with
---     | x +> xs, y +> ys =>
---       have h' : xs + ys = max _ ∧ y = !x := by
---         cases x <;> cases y
---         · simp [cons_add_cons, incr] at h;
---           rw [cons_eq_max] at h; simp [true_eq_one] at h
---         · simp [cons_add_cons, incr] at h;
---           rw [cons_eq_max] at h; refine' ⟨h.left, rfl⟩
---         · simp [cons_add_cons, incr, succ] at h;
---           rw [cons_eq_max] at h; refine' ⟨h.left, rfl⟩
---         · simp [cons_add_cons, incr, succ] at h;
---           rw [cons_eq_max] at h; simp at h
---       rw [h'.right, nof_iff_not_overflow]
---       unfold Overflow
---       simp only [Bits.toNat]
---       rw [not_le]
---       have hrw :
---         2 * toNat xs + x.toNat + (2 * toNat ys + (!x).toNat) =
---           2 * (toNat xs + toNat ys) + 1 := by
---         rw [Nat.mul_add, Nat.add_assoc, Nat.add_assoc]
---         simp; rw [Nat.add_comm, Nat.add_assoc]
---         cases x <;> rfl
---       rw [hrw, Nat.pow_succ, Nat.mul_comm (_ ^ _), Nat.lt_floor_left (by simp)]
---       apply Nat.mul_lt_mul_of_pos_left _ (by simp)
---       apply ih  _ _ h'.left
---
--- lemma Bits.cons_Overflow_cons {k} {xs ys : Bits k} {x y} (h : xs ↟ ys) : (x +> xs) ↟ (y +> ys) := by
---   simp [Overflow, Bits.toNat, Nat.pow_succ, Nat.mul_comm]
---   apply Nat.le_trans <| Nat.mul_le_mul_left 2 h
---   simp [Nat.mul_add]; rw [Nat.add_assoc, Nat.mul_comm]
---   simp; apply Nat.le_trans _ <| Nat.le_add_left _ _
---   rw [Nat.mul_comm]; apply Nat.le_add_right
---
--- lemma Bits.of_cons_nof_cons {k} {xs ys : Bits k} {x y} :
---     Nof (x +> xs) (y +> ys) → Nof xs ys := by
---   simp [nof_iff_not_overflow]; apply mt cons_Overflow_cons
---
--- lemma Bits.add_toNat {k} (xs ys : Bits k) (h : Nof xs ys) :
---     (xs + ys).toNat = xs.toNat + ys.toNat := by
---   induction k with
---   | zero => simp [nil_toNat]
---   | succ k ih =>
---     match xs, ys with
---     | x +> xs, y +> ys =>
---       by_cases h_eq : (xs + ys) +> y = max _
---       · rw [cons_eq_max] at h_eq
---         cases x
---         · rw [cons_add_cons]
---           simp only [incr, id, toNat]
---           rw [ih _ _ <| nof_of_add_eq_max _ _ h_eq.left]
---           rw [h_eq.right]
---           simp [Bool.one_toNat]
---           rw [Nat.mul_add, Nat.add_assoc]
---         · cases h_eq.right
---           simp [Nof, toNat, Bool.one_toNat] at h
---           have h_rw : 2 * xs.toNat + 1 + (2 * ys.toNat + 1) = 2 ^ k * 2 := by
---             rw [Nat.mul_comm _ 2, ← max_toNat_succ, ← h_eq.left]
---             rw [ih _ _ <| nof_of_add_eq_max _ _ h_eq.left]; omega
---           rw [h_rw, Nat.pow_succ] at h; simp [lt_irrefl] at h
---       · simp [cons_add_cons]
---         rw [incr_toNat_assoc _ _ h_eq]; simp [toNat]
---         rw [ih _ _ <| of_cons_nof_cons h, Nat.mul_add]
---         rw [Nat.add_assoc, Nat.add_assoc, Nat.add_assoc]
---         apply congr_arg (2 * xs.toNat + ·)
---         rw [← Nat.add_assoc, Nat.add_comm]
---
 
 lemma Bool.beq_eq_true (a b : Bool) : ((a == b) = true) = (a = b) := by
   cases a <;> cases b <;> simp
@@ -1801,41 +1009,6 @@ lemma Bits.toNat_sub_eq_of_le {k} (xs ys : Bits k) (h : ys ≤ xs) :
     (xs - ys).toNat = xs.toNat - ys.toNat := by
   rw [toNat_sub]; rw [← not_lt, lt_iff_lt'] at h; simp [h]
 
--- lemma Bits.sub_toNat {k} (xs ys : Bits k) (h : ys ≤ xs) :
---     (xs - ys).toNat = xs.toNat - ys.toNat := by
---   induction k with
---   | zero => simp [nil_toNat]
---   | succ k ih =>
---     match xs, ys with
---     | x +> xs, y +> ys =>
---       by_cases hd : (xs - ys) +> x = 0
---       · rw [cons_eq_zero_iff] at hd
---         have h_eq : xs = ys := by
---           have h := congr_arg (λ zs => zs + ys) hd.left
---           simp [sub_add_cancel, zero_add] at h; exact h
---         have h_eq' : y = 0 := by
---           rw [h_eq, hd.right, cons_le_cons] at h
---           simp [Bits.lt_irrefl] at h
---           cases y
---           · apply false_eq_zero
---           · simp [LE.le] at h
---         rw [h_eq, h_eq', hd.right, sub_self, Nat.sub_self, zero_toNat]
---       · rw [cons_sub_cons]
---         rw [decr_toNat_assoc _ _ hd]
---         simp only [toNat]; rw [cons_le_cons] at h
---         rcases h with h | h
---         · rw [ih _ _ <| Bits.le_of_lt h]
---           rw [Nat.mul_sub_left_distrib, Nat.sub_add_eq]
---           apply congr_arg₂ _ _ rfl
---           rw [← Nat.sub_add_comm]
---           rw [Nat.mul_le_mul_iff (by simp)]
---           apply Nat.le_of_lt <| toNat_lt_toNat _ _ h
---         · rw [h.left, sub_self, zero_toNat, Nat.mul_zero, Nat.zero_add]
---           rw [Nat.add_comm, Nat.sub_add_eq]
---           rw [Nat.add_sub_assoc <| Nat.le_refl _]
---           rw [Nat.sub_self, Nat.add_zero]
---
-
 lemma Bits.append_eq_append_iff {m n} {xs ys : Bits m} {xs' ys' : Bits n} :
     xs ++ xs' = ys ++ ys' ↔ (xs = ys ∧ xs' = ys') := by
   revert xs xs' ys ys' n
@@ -1878,16 +1051,6 @@ lemma toBits_toBytes {n} (xs : Bits (8 * n)) :
   · apply toBits'_toBytes
   · rw [List.length_reverse, Bits.length_toBytes]
 
-
-
-
-
-
-
---def Bits.succ : ∀ {n}, Bits n →  Bits n
---  | 0, ⦃⦄ => ⦃⦄
---  | _ + 1, x +> xs => (x != xs.isMax) +> xs.succ
-
 lemma Bits.succ_cons {n} (x) (xs : Bits n) :
      (x +> xs).succ = (x != xs.isMax) +> xs.succ := rfl
 
@@ -1898,15 +1061,6 @@ lemma Bits.append_eq_max_iff {m n} (xs : Bits m) (ys : Bits n) :
   | cons x xs ih =>
     rw [cons_append]; conv => lhs; rhs; apply (@max_eq_cons (n + _))
     rw [cons_eq_cons, ih, max_eq_cons, cons_eq_cons, and_assoc]
-
--- lemma Bits.zero_append_zero {m n} :
---     (0 : Bits m) ++ (0 : Bits n) = (0 : Bits (n + m)) := by
---   induction m with
---   | zero => rfl
---   | succ m ih =>
---     rw [zero_eq_append]
---     --simp [zero]; rw [cons_append, ih]
-
 
 lemma Bits.max_append_max {m n} :
     max m ++ max n = max (n + m) := by
@@ -1929,23 +1083,6 @@ lemma Bits.succ_append {m n} (xs : Bits m) (ys : Bits n) :
     · simp [h_rw, cons_append]
     · simp [h_rw, mt (eq_max_iff_isMax _).mpr h, cons_append]
     · simp [h_rw, cons_append]
-
--- lemma Bits.succ_append {m n} (xs : Bits m) (ys : Bits n) :
---     (xs ++ ys).succ = incr (if ys = max _ then 1 else 0) xs ++ ys.succ := by
---   induction ys with
---   | nil => rw [if_pos nil_eq_nil]; rfl
---   | cons ys y ih =>
---     cases y <;> simp only [succ]
---     · rw [if_neg]; rfl; simp [cons_eq_max]
---     · apply congrArg₂ _ (Eq.trans ih _) rfl
---       by_cases h : ys = max _
---       · rw [if_pos h, if_pos]; rfl
---         simp [cons_eq_max, h, Bool.one]
---       · rw [if_neg h, if_neg]; rfl
---         simp [cons_eq_max, h]
---
--- lemma Bits.succ_append_eq_of_ne {m n} (xs : Bits m) (ys : Bits n) (h : ys ≠ max _) :
---     (xs ++ ys).succ = xs ++ ys.succ := by rw [succ_append, if_neg h]; rfl
 
 lemma Bits.toBytes_eq_cons {n} (b : Byte) {xs : Bits (8 * n)} :
     @toBytes (n + 1) (b ++ xs) = b :: toBytes xs := by
@@ -1973,127 +1110,9 @@ lemma Bits.toBytes_eq_append {m n} {xs : Bits (8 * m)} {ys : Bits (8 * n)} :
     conv => rhs; lhs; arg 1; apply h_rw.symm
     rw [fappend_eq_append, toBytes_eq_cons, ih, toBytes_eq_cons, List.cons_append]
 
--- lemma Bits.max_eq_append {n} : (max (n + 1) : Bits (n + 1)) = 1 +> (max _ : Bits n) := rfl
-
--- lemma Bits.max_eq_append {n} : (max _ : Bits (n + 1)) = (max _ : Bits n) +> 1 := rfl
---
--- lemma Bits.append_eq_max {m n} {xs : Bits m} {ys : Bits n} :
---     xs ++ ys = max (m + n) ↔ xs = max m ∧ ys = max n := by
---   induction ys with
---   | nil => constructor <;> intro h; refine ⟨h, rfl⟩; apply h.left
---   | cons ys y ih =>
---     rename Nat => k; rw [append_cons, max_eq_append]
---     conv => lhs; rhs; apply (@max_eq_append (m + k)).symm
---     simp [max_eq_append]; rw [ih, and_assoc]
---
--- def Bytes.append : Bytes → Bytes → Bytes
---   | xs, [] => xs
---   | xs, ys :> y => append xs ys :> y
---
--- instance : HAppend Bytes Bytes Bytes := ⟨Bytes.append⟩
---
--- def Bytes.mem : Bytes → Byte → Prop
---   | [], _ => False
---   | bs :> b, b' => mem bs b' ∨ b = b'
---
--- instance : Membership Byte Bytes := ⟨Bytes.mem⟩
---
 abbrev Bytes.Zero : Bytes → Prop := List.Forall (· = 0)
--- | [] => True
--- | x :: xs => x = 0 ∧ zero xs
 
--- lemma Bytes.zero_of_sig_eq_nil {bs : Bytes} : bs.sig = [] → bs.zero := by
---   induction bs with
---   | nil => intro _; constructor
---   | cons bs b ih =>
---     simp [sig]
---     rcases eq_nil_or_eq_cons bs.sig with h_nil | h_cons
---     · simp [h_nil]; intro h; refine ⟨ih h_nil, h⟩
---     · rcases h_cons with ⟨bs', b, h⟩; simp [h]
---
--- lemma Bytes.append_cons {xs ys : Bytes} {y} : xs ++ (ys :> y) = ((xs ++ ys) :> y) := by
---   simp [HAppend.hAppend, append]
---
--- lemma Bytes.append_inj' {xs₁ xs₂ ys₁ ys₂ : Bytes} :
---     xs₁ ++ xs₂ = ys₁ ++ ys₂ →
---     xs₂.length = ys₂.length →
---     xs₁ = ys₁ ∧ xs₂ = ys₂ := by
---   revert ys₂
---   induction xs₂ with
---   | nil =>
---     intros ys₂ h_eq h_len
---     cases ys₂ with
---     | nil => refine' ⟨h_eq, rfl⟩
---     | cons _ _ => cases h_len
---   | cons xs₂ x ih =>
---     intros ys₂ h_eq h_len
---     cases ys₂ with
---     | nil => cases h_len
---     | cons ys₂ y =>
---       simp [append_cons] at h_eq
---       rcases h_eq with ⟨h_eq, ⟨_⟩⟩
---       simp [length] at h_len
---       simp; apply ih h_eq h_len
---
--- lemma Bytes.length_append (xs ys : Bytes) : (xs ++ ys).length = xs.length + ys.length := by
---   induction ys with
---   | nil => rfl
---   | cons ys y ih =>
---     simp [append_cons, length]
---     rw [← Nat.add_assoc, ← ih]; rfl
---
--- lemma Bytes.append_inj {xs₁ xs₂ ys₁ ys₂ : Bytes}
---     (h_eq : xs₁ ++ xs₂ = ys₁ ++ ys₂)
---     (h_len : xs₁.length = ys₁.length) : xs₁ = ys₁ ∧ xs₂ = ys₂ := by
---   apply append_inj' h_eq
---   apply @Nat.add_left_cancel ys₁.length
---   have h := congrArg length h_eq
---   simp [length_append, h_len] at h; rw [h]
---
--- lemma Bytes.prefix_unique {xs ys zs : Bytes}
---     (h_len : xs.length = ys.length)
---     (h_xs : xs <<+ zs)
---     (h_ys : ys <<+ zs) : xs = ys := by
---   rcases h_xs with ⟨sfx, h⟩
---   rcases h_ys with ⟨sfx', h'⟩
---   apply And.left <| append_inj (Eq.trans h.symm h') h_len
---
--- lemma Bytes.singleton_inj {x y} (h : [x] = [y]) : x = y := by cases h; rfl
---
--- lemma Bytes.append_assoc (as bs cs : Bytes) : as ++ bs ++ cs = as ++ (bs ++ cs) := by
---   induction cs with
---   | nil => rfl
---   | cons cs c ih => simp [append_cons, ih]
---
--- lemma Bytes.prefix_trans {xs ys zs : Bytes}
---     (h : xs <<+ ys) (h' : ys <<+ zs) : xs <<+ zs := by
---   rcases h with ⟨sfx, h_sfx⟩
---   rcases h' with ⟨sfx', h_sfx'⟩
---   refine' ⟨sfx ++ sfx', _⟩
---   rw [h_sfx', h_sfx]
---   apply append_assoc
---
--- lemma Bytes.length_eq_zero {xs : Bytes} : xs.length = 0 ↔ xs = [] := by
--- cases xs <;> simp [length]
---
--- lemma Bytes.split_nil {xs ys : Bytes} : (xs <++ [] ++> ys) ↔ (xs = [] ∧ ys = []) := by
---   match xs with
---   | [] =>
---     match ys with
---     | [] => simp; rfl
---     | ys :> y => simp; intro h; cases h
---   | xs :> x => cases ys <;> {simp; intro h; cases h}
---
--- lemma Bytes.prefix_nil {xs : Bytes} : xs <<+ [] ↔ xs = [] := by
---   constructor <;> intro h
---   · rcases h with ⟨ys, h⟩; rw [split_nil] at h; apply h.left
---   · rw [h]; refine ⟨[], rfl⟩
---
--- lemma Bytes.length_snoc {xs x} : length ([x] ++ xs) = xs.length + 1 := by
---   simp [length_append, Nat.add_comm, length]
-
-
-instance {ξ : Type u} {ρ : ξ → Prop} {xs : List ξ} --[dC : Decidable c]
+instance {ξ : Type u} {ρ : ξ → Prop} {xs : List ξ}
     [d : ∀ x : ξ, Decidable (ρ x)] : Decidable (xs.Forall ρ) := by
   induction xs with
   | nil => apply instDecidableTrue
@@ -2101,120 +1120,12 @@ instance {ξ : Type u} {ρ : ξ → Prop} {xs : List ξ} --[dC : Decidable c]
 
 def Bytes.Max (bs : Bytes) : Prop := bs.Forall (· = .max 8)
 
-lemma Bytes.max_cons (b) (bs : Bytes) :
-    Max (b :: bs) ↔ (b = Bits.max 8 ∧ Max bs) := by
-  simp only [Max, List.forall_cons]
-
-
 instance (bs : Bytes) : Decidable bs.Max := by
   unfold Bytes.Max; infer_instance
 
 def Bytes.succ : Bytes → Bytes
   | [] => []
   | b :: bs => (if Max bs then b.succ else b) :: succ bs
-
--- def Bytes.succ : Bytes → Bytes
---   | [] => []
---   | xs :> x =>
---     if x = Ox xF xF
---     then succ xs :> 0
---     else xs :> x.succ
---
--- lemma Bytes.succ_cons_max_eq {xs} : (xs :> Ox xF xF).succ = succ xs :> 0 := by
---   simp only [Bytes.succ]; rw [if_pos cst]
---
--- lemma Bytes.succ_cons_eq_of_ne {xs x} (h : x ≠ Ox xF xF) : (xs :> x).succ = xs :> x.succ := by
---   unfold Bytes.succ; rw [if_neg h]
---
-
---   | [] => True
---   | xs :> x => max xs ∧ x = Ox xF xF
-
-lemma Bytes.toBits'_eq_zero {n} {xs : Bytes} (h : xs.Zero) :
-    toBits' n xs = 0 := by
-  induction n generalizing xs h with
-  | zero => rfl
-  | succ n ih =>
-    match xs with
-    | [] => simp [toBits']; rw [ih cst]; rfl
-    | x :: xs =>
-      simp [toBits', Bytes.Zero] at *
-      simp [h.left, ih h.right]; rfl
-
-lemma Bytes.max_iff_toBits'_eq_max {bs : Bytes} :
-     bs.Max ↔ toBits' bs.length bs = Bits.max (8 * bs.length) := by
-  induction bs with
-  | nil => apply iff_of_true cst rfl
-  | cons xs bs ih =>
-    simp [max_cons, toBits']; rw [ih]
-    apply (Bits.append_eq_max_iff xs (toBits' bs.length bs)).symm
-
-lemma Bytes.toBits'_eq_max {n} {xs : Bytes} (h : xs.Max) (h' : n ≤ xs.length):
-    toBits' n xs = Bits.max (8 * n) := by
-  induction n generalizing xs h with
-  | zero => rfl
-  | succ n ih =>
-    match xs with
-    | [] => simp [List.length] at h'
-    | x :: xs =>
-      simp [List.length] at h'; simp [max_cons] at h; simp [toBits']
-      rw [h.left, ih h.right h', Bits.max_append_max]; rfl
-
-lemma List.forall_append {ξ : Type u} (π : ξ → Prop) (xs ys : List ξ)
-    (h : xs.Forall π) (h' : ys.Forall π) : (xs ++ ys).Forall π := by
-  induction xs with
-  | nil => apply h'
-  | cons x xs ih => simp [Forall] at *; refine' ⟨h.left, ih h.right⟩
-
-lemma List.forall_reverse {ξ : Type u} (π : ξ → Prop) (xs : List ξ)
-    (h : xs.Forall π) : xs.reverse.Forall π := by
-  induction xs with
-  | nil =>  constructor
-  | cons x xs ih =>
-    simp [reverse_cons] at *
-    apply forall_append _ _ _ (ih h.right)
-    simp [h.left]
-
-lemma List.forall_replicate {ξ : Type u} (π : ξ → Prop) (n) (x) (h : π x) :
-    (replicate n x).Forall π := by
-  induction n with
-  | zero => simp
-  | succ n ih => simp [replicate, h, ih]
-
-lemma List.forall_takeD {ξ : Type u} (π : ξ → Prop) (n) (xs : List ξ) (x)
-    (h : xs.Forall π) (h' : π x) : (xs.takeD n x).Forall π := by
-  induction n generalizing xs with
-  | zero => simp [takeD]
-  | succ n ih =>
-    match xs with
-    | [] => simp [h', forall_replicate]
-    | x :: xs => simp at *; refine ⟨h.left, ih _ h.right⟩
-
-lemma Bytes.toBits_eq_zero {n} {xs : Bytes} (h : xs.Zero) : toBits n xs = 0 := by
-  apply toBits'_eq_zero (List.forall_reverse _ _ _)
-  apply List.forall_takeD
-  · apply List.forall_reverse _ _ h
-  · rfl
-
--- lemma Bytes.of_toBits_succ_eq_toBits_succ {n} {bs bs' : Bytes} :
---     toBits (n + 1) bs = toBits (n + 1) bs' → toBits n bs = toBits n bs' := by
---   induction n generalizing bs bs' with
---   | zero => intro _; rfl
---   | succ n ih =>
---     match bs, bs' with
---     | nil, nil => simp [toBits]
---     | nil, cons bs' b' =>
---       simp [toBits]; intro h
---       rw [Bits.append_eq_append_iff] at h
---       rw [@ih nil bs' h.left, h.right]
---     | cons bs b, nil =>
---       simp [toBits]; intro h
---       rw [Bits.append_eq_append_iff] at h
---       rw [@ih nil bs h.left.symm, h.right]
---     | cons bs b, cons bs' b' =>
---       simp [toBits]; intro h
---       rw [Bits.append_eq_append_iff] at h
---       rw [ih h.left, h.right]
 
 lemma List.takeD_concat {ξ : Type u} (n) (xs : List ξ) (y) :
     takeD n (xs.concat y) y = takeD n xs y := by
@@ -2244,159 +1155,6 @@ lemma Bytes.sig_toBits {n} (bs : Bytes) : bs.sig.toBits n = bs.toBits n := by
       · rw [decide_eq_true rfl]
     · rw [List.dropWhile_cons_of_neg _]
       rw [decide_eq_false hb]; simp
-
--- lemma Bytes.sig_toBits {n} (bs : Bytes) : bs.sig.toBits n = bs.toBits n := by
---   induction bs with
---   | nil => rfl
---   | cons bs b ih =>
---     rcases eq_nil_or_eq_cons bs.sig with h_nil | h_cons
---     · simp [sig]; simp [h_nil]
---       by_cases hb : b = 0
---       · rw [if_pos hb]
---         rw [@toBits_eq_zero n (bs :> b) ⟨zero_of_sig_eq_nil h_nil, hb⟩]
---         apply toBits_eq_zero; constructor
---       · rw [if_neg hb]
---         cases n with
---         | zero => rfl
---         | succ n =>
---           simp [toBits]
---           rw [← of_toBits_succ_eq_toBits_succ ih, h_nil]
---     · rcases h_cons with ⟨bs', b', h_sig⟩
---       simp [sig]; simp [h_sig]
---       cases n with
---       | zero => rfl
---       | succ n =>
---         simp [toBits]
---         rw [← of_toBits_succ_eq_toBits_succ ih, h_sig]
---
--- lemma Bytes.nil_append {xs} : [] ++ xs = xs := by
---   induction xs with
---   | nil => rfl
---   | cons xs x ih => rw [append_cons, ih]
-lemma Bits.succ_max {k} : succ (max k) = 0 := by
-  induction k with
-  | zero => rfl
-  | succ k ih => simp [max, succ, max_isMax, ih]; rfl
-
-lemma Bytes.zero_succ_of_max {bs : Bytes} (h : Max bs) : (succ bs).Zero := by
-  induction bs with
-  | nil => constructor
-  | cons b bs ih =>
-    rw [max_cons] at h
-    simp [succ, Zero, h.left, h.right, ih h.right, Bits.succ_max]
-
-lemma Bytes.toBits'_succ  {bs : Bytes} :
-    bs.succ.toBits' bs.length = (bs.toBits' bs.length).succ := by
-  induction bs with
-  | nil => rfl
-  | cons b bs ih =>
-    simp only [Bytes.succ, toBits', Bits.succ_append, List.length]
-    rw [ih]; by_cases h' : Max bs
-    · simp [h', max_iff_toBits'_eq_max.mp h']
-    · simp [h', mt max_iff_toBits'_eq_max.mpr h']
-
-
--- lemma Bytes.toBits_succ {n} {bs : Bytes} (h : ¬ bs.Max) :
---     bs.succ.toBits n = (bs.toBits n).succ := by
---   unfold toBits
---   have h_rw := @toBits'_succ (List.takeD n bs.reverse 0).reverse
---   rw [List.length_reverse, List.takeD_length] at h_rw
---   rw [← h_rw]
---   apply congr_arg
-
-
-
-
-
-
-
-
---  induction n generalizing bs with
---  | zero => rfl
---  | succ n ih =>
---    match bs with
---    | [] => cases (h cst)
---    | b :: bs =>
---      simp only [Bytes.succ, toBits]
---
-
-
-
--- lemma Bytes.toBits_succ {n} {xs : Bytes} :
---     ¬ xs.max → Bytes.toBits n xs.succ = (Bytes.toBits n xs).succ := by
---   revert xs
---   induction n with
---   | zero => intros _ _; simp [Bytes.toBits]; rfl
---   | succ n ih =>
---     intro xs h
---     match xs with
---     | [] => cases h (by constructor)
---     | xs :> x =>
---       cases em (x = Ox xF xF) with
---       | inl hx =>
---         rw [hx]; simp [Bytes.succ, Bytes.toBits, Bits.succ]
---         rw [ih _]; rfl; intro hc; apply h; refine ⟨hc, hx⟩
---       | inr hx =>
---         rw [Bytes.succ_cons_eq_of_ne hx]; simp [Bytes.toBits]
---         rw [Bits.succ_append_eq_of_ne _]; apply hx
---
-
-lemma Bits.eq_max_iff_max_toBytes {k : ℕ} (xs : Bits (8 * k)) :
-    xs = max (8 * k) ↔ xs.toBytes.Max := by
-  induction k with
-  | zero => cases xs; apply iff_of_true rfl cst
-  | succ k ih =>
-    rw [← @prefix_append_suffix (8 * k) 8 xs, toBytes_eq_cons]
-    conv => lhs; rhs; apply (@max_append_max 8 (8 * k)).symm
-    rw [append_eq_append_iff, ih]; simp [Bytes.Max]
-
-lemma Bits.toBytes_succ {n} :
-    ∀ {xs : Bits (8 * n)}, xs.succ.toBytes = Bytes.succ xs.toBytes := by
-  induction n with
-  | zero => simp [Nat.mul_zero]; intro xs; cases xs; rfl
-  | succ n ih =>
-    simp [Nat.mul_succ]; intro xs
-    rw [← @prefix_append_suffix (8 * n) 8 xs, toBytes_eq_cons]
-    simp [Bytes.succ]
-    rw [← @ih xs.suffix, succ_append, toBytes_eq_cons]
-    split
-    · simp [(eq_max_iff_max_toBytes _).mp asm]
-    · simp [mt (eq_max_iff_max_toBytes _).mpr asm]
-
-
-
-
-
-
-
-
-
-
-
-
-
-
-
-
-
--- lemma Bits.toBytes_succ {n} {xs : Bits (8 * n)} :
---     xs.succ.toBytes = Bytes.succ xs.toBytes := by
---   revert xs
---   induction n with
---   | zero => simp [Nat.mul_zero]; intro xs; cases xs; rfl
---   | succ n ih =>
---     simp [Nat.mul_succ]; intro xs
---     rw [← @Bits.prefix_append_suffix (8 * n) 8 xs]
---     cases em (xs.tail = Ox xF xF) with
---     | inl h =>
---       rw [h]; simp only [Bits.toBytes]
---       apply Eq.trans _ <| Eq.symm Bytes.succ_cons_max_eq
---       rw [ih]; rfl
---     | inr h =>
---       rw [Bits.succ_append_eq_of_ne _]
---       simp [Bits.toBytes_append]
---       rw [Bytes.succ_cons_eq_of_ne h]
---       apply h
 
 def List.drop? {ξ : Type u} : Nat → List ξ → Option (List ξ)
   | 0, xs => some xs
@@ -2437,14 +1195,6 @@ lemma List.slice?_cons {ξ : Type u} (x) (xs : List ξ) (m n : Nat) :
 
 def List.sliceD {ξ : Type u} [Zero ξ] (xs : List ξ) (m n : Nat) (x : ξ) : List ξ :=
   takeD n (drop m xs) x
-
--- lemma List.take?_eq_some_cons {ξ : Type u}
---     (n : ℕ) (x : ξ) (xs : List ξ) (y : ξ) (ys : List ξ) :
---     take? (n + 1) (x :: xs) = some (y :: ys) ↔ x = y ∧ take? n xs = some ys := by
---   simp only [take?]
---   cases take? n xs with
---   | none => simp
---   | some zs => simp
 
 lemma List.slice?_eq_cons_iff {ξ : Type u} {xs : List ξ} {m n : Nat} {y} {ys} :
     slice? xs m (n + 1) = some (y :: ys) ↔
@@ -2489,10 +1239,6 @@ lemma List.length_slice? {ξ : Type u} {xs} {m n : Nat} {ys : List ξ} :
     slice? xs m n = some ys → n = ys.length := by
   unfold slice?; cases xs.drop? m <;> simp; apply length_take?
 
-lemma List.get?_eq_of_slice?_eq {ξ : Type u} {xs : List ξ} {m n : Nat} {y} {ys} :
-    slice? xs m (n + 1) = some (y :: ys) → get? xs m = some y := by
-  rw [slice?_eq_cons_iff]; apply And.left
-
 lemma List.get?_eq_of_slice {ξ : Type u} {xs : List ξ} {m : Nat} {y} {ys} :
     Slice xs m (y :: ys) → get? xs m = some y := by
   rw [slice_cons_iff]; apply And.left
@@ -2524,17 +1270,9 @@ lemma List.of_slice?_eq_append {ξ : Type u} {xs : List ξ}
   revert h; unfold slice?; rw [Nat.add_comm, drop?_add]
   cases xs.drop? m <;> simp; rename List ξ => xs'; apply of_take?_eq_append
 
-lemma List.slice?_eq_prefix {ξ : Type u} {xs : List ξ}
-    {m n : Nat} {ys zs} (h : slice? xs m n = some (ys ++ zs)) :
-    slice? xs m ys.length = some ys := (of_slice?_eq_append h).left
-
 lemma List.slice_prefix {ξ : Type u} {xs : List ξ}
     {m : Nat} {ys zs} (h : Slice xs m (ys ++ zs)) : Slice xs m ys := by
   rcases h with ⟨n, h⟩; refine ⟨_, (of_slice?_eq_append h).left⟩
-
--- lemma List.slice?_eq_suffix {ξ : Type u} {xs : List ξ}
---     {m n : Nat} {ys zs} (h : slice? xs m n = some (ys ++ zs)) :
---     slice? xs (m + ys.length) zs.length = some zs := (of_slice?_eq_append h).right
 
 lemma List.slice_suffix {ξ : Type u} {xs : List ξ} {m : Nat} {ys zs}
     (h : Slice xs m (ys ++ zs)) : Slice xs (m + ys.length) zs := by
@@ -2550,16 +1288,6 @@ lemma List.get?_length_ne_some {ξ : Type y} {xs : List ξ} {y} :
 lemma List.not_slice_length {xs} {y} {ys : List ξ} :
     ¬ Slice xs xs.length (y :: ys) := by simp [slice_cons_iff]
 
---   intro h; rcases h with ⟨pfx, sfx, h_split, h_pfx, h_len⟩
---   have h_sfx : sfx = [] := by
---     have h := congrArg Bytes.length h_split
---     rw [Bytes.length_append, h_len] at h
---     have h' := Nat.eq_sub_of_add_eq' h.symm; simp at h'
---     rw [← Bytes.length_eq_zero, h']
---   rw [h_sfx, Bytes.prefix_nil] at h_pfx; cases h_pfx
-
-  --rcases h with ⟨n, h⟩; refine ⟨_, (of_slice?_eq_append h).left⟩
-
 lemma List.take?_length {ξ : Type u} (xs : List ξ) :
     take? xs.length xs = some xs := by
   induction xs with
@@ -2569,57 +1297,10 @@ lemma List.take?_length {ξ : Type u} (xs : List ξ) :
 lemma List.slice_refl {ξ : Type u} (xs : List ξ) : List.Slice xs 0 xs := by
   refine' ⟨xs.length, _⟩; simp [slice?, drop?, take?_length]
 
--- def sliceFill (bs : Bytes) (loc sz : Nat) (sc : Bytes) : Prop :=
---   (slice bs loc sc ∧ sc.length = sz) ∨
---   ∃ pfx sfx zrs,
---     (pfx <++ bs ++> sfx) ∧
---     (sfx <++ sc ++> zrs) ∧
---     pfx.length = loc ∧
---     sc.length = sz ∧
---     Bytes.zero zrs
---
--- lemma slice_unique {xs ys zs : Bytes} {k}
---     (h_eq : ys.length = zs.length)
---     (h_ys : slice xs k ys)
---     (h_zs : slice xs k zs) : ys = zs := by
---   simp [slice] at h_ys
---   rcases h_ys with ⟨pfx, sfx, h_split, h_pfx, h_len⟩
---   rcases h_zs with ⟨pfx', sfx', h_split', h_pfx', h_len'⟩
---   cases
---     And.right <|
---       Bytes.append_inj
---         (Eq.trans h_split.symm h_split')
---           (Eq.trans h_len h_len'.symm)
---   apply Bytes.prefix_unique h_eq h_pfx h_pfx'
---
--- lemma slice_singleton_unique {xs : Bytes} {k} {x y}
---     (h : slice xs k [x]) (h' : slice xs k [y]) : x = y := by
---   apply Bytes.singleton_inj <| slice_unique _ h h'; rfl
---
--- lemma slice_prefix {xs ys zs : Bytes} {k} (h : slice xs k (ys ++ zs)) :
---     slice xs k ys := by
---   rcases h with ⟨pfx, sfx, h_xs, h_sfx, h_len⟩
---   refine' ⟨pfx, sfx, h_xs, _, h_len⟩
---   apply Bytes.prefix_trans (pref_append _ _) h_sfx
---
--- lemma slice_suffix {xs ys zs : Bytes} {k} (h : slice xs k (ys ++ zs)) :
---     slice xs (k + ys.length) zs := by
---   rcases h with ⟨pfx, sfx, h_xs, h_sfx, h_len⟩
---   rcases h_sfx with ⟨sfx', h_sfx⟩
---   refine' ⟨pfx ++ ys, zs ++ sfx', _, pref_append _ _, _⟩
---   · rw [h_xs, h_sfx]; unfold Split; simp [← Bytes.append_assoc]
---   · rw [← h_len]; apply Bytes.length_append
---
 lemma List.append_slice_suffix {ξ : Type y} {xs ys : List ξ} :
     Slice (xs ++ ys) xs.length ys := by
   have h := slice_suffix <| slice_refl <| xs ++ ys
   rw [Nat.zero_add] at h; exact h
-
-lemma zero_toBytes_zero {n} : (@Bits.toBytes n 0).Zero := by
-  induction n with
-  | zero => constructor
-  | succ n ih => simp [Bits.toBytes, Bytes.Zero]; refine ⟨rfl, ih⟩
-
 
 lemma toBytes_zero_eq_replicate_zero {n} :
     (@Bits.toBytes n 0) = List.replicate n (0 : Byte) := by
@@ -2645,50 +1326,10 @@ lemma Bits.zero_ne_succ {n} :
 lemma Bits.add_comm {n} {xs ys : Bits n} : xs + ys = ys + xs := by
   apply toNat_inj; simp [toNat_add]; rw [Nat.add_comm, overflow_comm]
 
-
-
-
-
-
-
-
-
-
---
--- #exit
---
---
---
---     rw [zero_eq_cons] at h
---     revert h;
---
---
---
---
---
---
---
---
---
---   --cases h
-
 lemma Bits.invert_zero_eq_max {n} : ~ (0 : Bits n) = max _ := by
   induction n with
   | zero => apply nil_eq_nil
   | succ n ih => rw [zero_eq_cons]; simp only [max, not]; rw [ih]; rfl
---
--- lemma Bits.max_and {n} {xs : Bits n} : and (max n) xs = xs := by
---   induction n with
---   | zero => apply nil_eq_nil
---   | succ n ih =>
---     cases xs with
---     | cons xs x =>
---       simp [max]
---       rw [cons_and_cons]
---       simp [Nat.add] at ih
---       rw [@ih xs]
---       cases x <;> rfl
-
 
 lemma Bits.zipWith_comm (f : Bool → Bool → Bool)
     (hf : ∀ x y, f x y = f y x) (n) :
@@ -2716,19 +1357,6 @@ lemma Bits.zero_and {n} {xs : Bits n} : and (0 : Bits n) xs = 0 := by
 lemma Bits.and_zero {n} {xs : Bits n} : and xs (0 : Bits n) = 0 := by
   rw [and_comm, zero_and]
 
--- lemma Bool.toNat_inj (x y : Bool) : x.toNat = y.toNat → x = y := by
---   cases x <;> cases y <;> simp
---
--- lemma Bits.toNat_inj {k} (xs ys : Bits k) (h : xs.toNat = ys.toNat) : xs = ys := by
---   induction k with
---   | zero => apply Bits.nil_eq_nil
---   | succ k ih =>
---     match xs, ys with
---     | x +> xs, y +> ys =>
---       simp [Bits.toNat] at h
---       cases Nat.eq_floor (Bool.toNat_lt _) (Bool.toNat_lt _) h
---       rw [ih xs ys asm, Bool.toNat_inj x y asm]
---
 lemma toBits_toNat {k : ℕ} {xs : Bits k} : Nat.toBits k (Bits.toNat xs) = xs := by
   apply Bits.toNat_inj; rw [toNat_toBits (Bits.toNat_lt_pow _)]
 
@@ -2737,25 +1365,161 @@ lemma Bits.of_toNat_le_toNat {k : ℕ} {xs ys : Bits k}
   have h' := Nat.toBits_le_toBits h (toNat_lt_pow _)
   rw [toBits_toNat, toBits_toNat] at h'; exact h'
 
--- lemma Bits.of_toNat_le_toNat {k : ℕ} {xs ys : Bits k}
---     (h : xs.toNat ≤ ys.toNat) : xs ≤ ys := by
---   have h' := toBits_le_toBits h (toNat_lt_pow _)
---   rw [toNat_toBits, toNat_toBits] at h'; exact h'
-
 lemma Bits.le_add_right {n} {xs ys : Bits n} (h : Nof xs ys) : xs ≤ xs + ys := by
   apply of_toNat_le_toNat; rw [toNat_add_eq_of_nof _ _ h]; apply Nat.le_add_right
 
-lemma Bits.add_zero {n} (xs : Bits n) : xs + 0 = xs := by
-  apply toNat_inj; rw [toNat_add]; simp [toNat_zero, overflow_zero]
+def Char.toHex : Char → Hex
+  | '0' => x0
+  | '1' => x1
+  | '2' => x2
+  | '3' => x3
+  | '4' => x4
+  | '5' => x5
+  | '6' => x6
+  | '7' => x7
+  | '8' => x8
+  | '9' => x9
+  | 'a' => xA
+  | 'b' => xB
+  | 'c' => xC
+  | 'd' => xD
+  | 'e' => xE
+  | 'f' => xF
+  | 'A' => xA
+  | 'B' => xB
+  | 'C' => xC
+  | 'D' => xD
+  | 'E' => xE
+  |  _  => xF
 
+def String.toBits : ∀ s : String, Bits (4 * s.length)
+  | ⟨[]⟩ => ⦃⦄
+  | ⟨c :: cs⟩ => Char.toHex c ++ toBits ⟨cs⟩
+abbrev Vec := Mathlib.Vector
 
+abbrev Qords : Type := Vec (Bits 64) 25
 
+def Char.toByte (c : Char) : Byte := Nat.toBits 8 c.toNat
+def String.toBytes (s : String) : Bytes := s.data.map Char.toByte
 
+def Bytes.toHex (bs : Bytes) : String :=
+  List.foldr (λ b s => Byte.toString b ++ s) "" bs
 
+def Bytes.toHexString (bs : Bytes) : String :=
+  "hex\"" ++ List.foldr (λ b s => Byte.toString b ++ s) "\"" bs
 
+def Bits.toHex {k : Nat} (xs : Bits (8 * k)) : String :=
+  Bytes.toHex <| Bits.toBytes xs
 
---   apply Nat.rec
---   · intros _; apply nil_eq_nil
---   · intros m ih xs; rcases xs with _ | ⟨xs, x⟩
---     rw [zero_eq_cons, cons_add_cons_zero, ih]
---
+def Qords.init : Qords := Mathlib.Vector.replicate 25 (.zero 64)
+
+def Qords.toString (ws : Qords) : String :=
+  let f : Fin 25 → String :=
+    λ k => @Bits.toHex 8 (ws.get k)
+  s!"{f 0} {f 1} {f 2} {f 3} {f 4}\n" ++
+  s!"{f 5} {f 6} {f 7} {f 8} {f 9}\n" ++
+  s!"{f 10} {f 11} {f 12} {f 13} {f 14}\n" ++
+  s!"{f 15} {f 16} {f 17} {f 18} {f 19}\n" ++
+  s!"{f 20} {f 21} {f 22} {f 23} {f 24}\n"
+
+def Qords.app (k : Nat) (f : Bits 64 → Bits 64) (ws : Qords) : Qords :=
+  ws.set k <| f <| ws.get k
+
+infixl:65 " ^^ " => Bits.xor
+
+def sha3rotl64 (xs : Bits 64) (y : Nat) : Bits 64 :=
+  Bits.or (xs.shl y) (xs.shr (64 - y))
+
+def theta'' (t : Bits 64) (i : Nat) : Nat → Qords → Qords
+  | 0, ws => ws
+  | j + 1, ws => theta'' t i j <| ws.app ((j * 5) + i) (· ^^ t)
+
+def theta' (bc : Vec (Bits 64) 5) : Nat → Qords → Qords
+| 0, ws => ws
+| i + 1, ws =>
+  let t : Bits 64 := bc.get (i + 4) ^^ sha3rotl64 (bc.get (i + 1)) 1
+  theta' bc i <| theta'' t i 5 ws
+
+def theta (ws : Qords) : Qords :=
+  let g : Fin 5 → Bits 64 :=
+    λ x => ws.get x ^^ ws.get (x + 5) ^^ ws.get (x + 10) ^^
+           ws.get (x + 15) ^^ ws.get (x + 20)
+  let bc : Vec (Bits 64) 5 := ⟨[g 0, g 1, g 2, g 3, g 4], rfl⟩
+  theta' bc 5 ws
+
+def keccakf_rndc : Vec (Bits 64) 24 :=
+  ⟨ [ "0000000000000001".toBits, "0000000000008082".toBits,
+      "800000000000808a".toBits, "8000000080008000".toBits,
+      "000000000000808b".toBits, "0000000080000001".toBits,
+      "8000000080008081".toBits, "8000000000008009".toBits,
+      "000000000000008a".toBits, "0000000000000088".toBits,
+      "0000000080008009".toBits, "000000008000000a".toBits,
+      "000000008000808b".toBits, "800000000000008b".toBits,
+      "8000000000008089".toBits, "8000000000008003".toBits,
+      "8000000000008002".toBits, "8000000000000080".toBits,
+      "000000000000800a".toBits, "800000008000000a".toBits,
+      "8000000080008081".toBits, "8000000000008080".toBits,
+      "0000000080000001".toBits, "8000000080008008".toBits ], rfl ⟩
+
+def keccakf_rotc : Vec Nat 24 :=
+  ⟨ [ 1, 3, 6, 10, 15, 21, 28, 36, 45, 55, 2, 14, 27,
+      41, 56, 8, 25, 43, 62, 18, 39, 61, 20, 44 ], rfl ⟩
+
+def keccakf_piln : Vec Nat 24 :=
+  ⟨ [ 10, 7, 11, 17, 18, 3, 5, 16, 8, 21, 24, 4,
+      15, 23, 19, 13, 12, 2, 20, 14, 22, 9, 6, 1 ], rfl ⟩
+
+def rhopiAux : Nat → Bits 64 → Qords → Qords
+  | 0, _, ws => ws
+  | k + 1, t, ws =>
+    let i := 23 - k
+    let j := keccakf_piln.get i
+    let ws' := ws.set j (sha3rotl64 t <| keccakf_rotc.get i)
+    rhopiAux k (ws.get j) ws'
+
+def rhopi (ws : Qords) : Qords := rhopiAux 24 (ws.get 1) ws
+
+def chi'' (ws : Qords) (bc : Vec (Bits 64) 5) (j : Nat) : Nat → Qords
+  | 0 => ws
+  | i + 1 =>
+    let ws' := ws.app (j + i) (·  ^^ (.and (bc.get (i + 1)).not (bc.get (i + 2))))
+    chi'' ws' bc j i
+
+def chi' (ws : Qords) : Nat → Qords
+  | 0 => ws
+  | k + 1 =>
+    let j := k * 5
+    let f : Nat → Bits 64 := λ x => ws.get (j + x)
+    let bc : Vec (Bits 64) 5 := ⟨[f 0, f 1, f 2, f 3, f 4], rfl⟩
+    let ws' : Qords := chi'' ws bc j 5
+    chi' ws' k
+
+def chi (ws : Qords) : Qords := chi' ws 5
+
+def iota (round : Nat) (ws : Qords) : Qords :=
+  ws.app 0 (· ^^ keccakf_rndc.get round)
+
+def kecaux : Nat → Qords → Qords
+| 0, ws => ws
+| n + 1, ws =>
+  kecaux n <| iota (23 - n) <| chi <| rhopi <| theta ws
+
+def keccakf (ws : Qords) : Qords := kecaux 24 ws
+
+def Qord.reverse (w : Bits 64) : Bits 64 :=
+  Bytes.toBits 8 (@Bits.toBytes 8 w).reverse
+
+def Bytes.keccak : Fin 17 → Bytes → Qords → Word
+| wc, b0 :: b1 :: b2 :: b3 :: b4 :: b5 :: b6 :: b7 :: bs, ws =>
+  let t : Bits 64 := Bytes.toBits 8 [b7, b6, b5, b4, b3, b2, b1, b0]
+  let ws' := ws.app wc (· ^^ t)
+  keccak (wc + 1) bs <| if wc = 16 then (keccakf ws') else ws'
+| wc, bs, ws =>
+  let t := Bytes.toBits' 8 ((bs ++ [Bits.one 8]).takeD 8 (.zero 8)).reverse
+  let s := "8000000000000000".toBits
+  let ws' := keccakf <| .app 16 (· ^^ s) <| .app wc (· ^^ t) ws
+  (Qord.reverse <| ws'.get 0) ++ (Qord.reverse <| ws'.get 1) ++
+  (Qord.reverse <| ws'.get 2) ++ (Qord.reverse <| ws'.get 3)
+
+def String.keccak (s : String) : Word :=
+  Bytes.keccak 0 s.toBytes Qords.init
